prefer plain subscript for notation;

thys/NormByEval/NBE.thy
@@ -21,10 +21,10 @@ text{* ML terms: *}
 
 datatype ml =
  -- "ML"
-  C_ML cname ("C\<^bsub>ML\<^esub>") (* ref to compiled code *)
-| V_ML ml_vname ("V\<^bsub>ML\<^esub>")
-| A_ML ml "(ml list)" ("A\<^bsub>ML\<^esub>")
-| Lam_ML ml ("Lam\<^bsub>ML\<^esub>")
+  C_ML cname ("C\<^sub>M\<^sub>L") (* ref to compiled code *)
+| V_ML ml_vname ("V\<^sub>M\<^sub>L")
+| A_ML ml "(ml list)" ("A\<^sub>M\<^sub>L")
+| Lam_ML ml ("Lam\<^sub>M\<^sub>L")
  -- "the universal datatype"
 | C\<^sub>U cname "(ml list)"
 | V\<^sub>U vname "(ml list)"
@@ -70,17 +70,17 @@ qed
 
 text{* Closed terms w.r.t.\ ML variables:*}
 
-fun closed_ML :: "nat \<Rightarrow> ml \<Rightarrow> bool" ("closed\<^bsub>ML\<^esub>") where
-"closed\<^bsub>ML\<^esub> i (C\<^bsub>ML\<^esub> nm) = True" |
-"closed\<^bsub>ML\<^esub> i (V\<^bsub>ML\<^esub> X) = (X<i)"  |
-"closed\<^bsub>ML\<^esub> i (A\<^bsub>ML\<^esub> v vs) = (closed\<^bsub>ML\<^esub> i v \<and> (\<forall>v \<in> set vs. closed\<^bsub>ML\<^esub> i v))" |
-"closed\<^bsub>ML\<^esub> i (Lam\<^bsub>ML\<^esub> v) = closed\<^bsub>ML\<^esub> (i+1) v" |
-"closed\<^bsub>ML\<^esub> i (C\<^sub>U nm vs) = (\<forall>v \<in> set vs. closed\<^bsub>ML\<^esub> i v)" |
-"closed\<^bsub>ML\<^esub> i (V\<^sub>U nm vs) = (\<forall>v \<in> set vs. closed\<^bsub>ML\<^esub> i v)" |
-"closed\<^bsub>ML\<^esub> i (Clo f vs n) = (closed\<^bsub>ML\<^esub> i f \<and> (\<forall>v \<in> set vs. closed\<^bsub>ML\<^esub> i v))" |
-"closed\<^bsub>ML\<^esub> i (apply v w) = (closed\<^bsub>ML\<^esub> i v \<and> closed\<^bsub>ML\<^esub> i w)"
+fun closed_ML :: "nat \<Rightarrow> ml \<Rightarrow> bool" ("closed\<^sub>M\<^sub>L") where
+"closed\<^sub>M\<^sub>L i (C\<^sub>M\<^sub>L nm) = True" |
+"closed\<^sub>M\<^sub>L i (V\<^sub>M\<^sub>L X) = (X<i)"  |
+"closed\<^sub>M\<^sub>L i (A\<^sub>M\<^sub>L v vs) = (closed\<^sub>M\<^sub>L i v \<and> (\<forall>v \<in> set vs. closed\<^sub>M\<^sub>L i v))" |
+"closed\<^sub>M\<^sub>L i (Lam\<^sub>M\<^sub>L v) = closed\<^sub>M\<^sub>L (i+1) v" |
+"closed\<^sub>M\<^sub>L i (C\<^sub>U nm vs) = (\<forall>v \<in> set vs. closed\<^sub>M\<^sub>L i v)" |
+"closed\<^sub>M\<^sub>L i (V\<^sub>U nm vs) = (\<forall>v \<in> set vs. closed\<^sub>M\<^sub>L i v)" |
+"closed\<^sub>M\<^sub>L i (Clo f vs n) = (closed\<^sub>M\<^sub>L i f \<and> (\<forall>v \<in> set vs. closed\<^sub>M\<^sub>L i v))" |
+"closed\<^sub>M\<^sub>L i (apply v w) = (closed\<^sub>M\<^sub>L i v \<and> closed\<^sub>M\<^sub>L i w)"
 
-fun closed_tm_ML :: "nat \<Rightarrow> tm \<Rightarrow> bool" ("closed\<^bsub>ML\<^esub>") where
+fun closed_tm_ML :: "nat \<Rightarrow> tm \<Rightarrow> bool" ("closed\<^sub>M\<^sub>L") where
 "closed_tm_ML i (r\<bullet>s) = (closed_tm_ML i r \<and> closed_tm_ML i s)" |
 "closed_tm_ML i (\<Lambda> t) = (closed_tm_ML i t)" |
 "closed_tm_ML i (term v) = closed_ML i v" |
@@ -88,15 +88,15 @@ fun closed_tm_ML :: "nat \<Rightarrow> tm \<Rightarrow> bool" ("closed\<^bsub>ML
 
 text{* Free variables: *}
 
-fun fv_ML :: "ml \<Rightarrow> ml_vname set" ("fv\<^bsub>ML\<^esub>") where
-"fv\<^bsub>ML\<^esub> (C\<^bsub>ML\<^esub> nm) = {}" |
-"fv\<^bsub>ML\<^esub> (V\<^bsub>ML\<^esub> X) = {X}"  |
-"fv\<^bsub>ML\<^esub> (A\<^bsub>ML\<^esub> v vs) = fv\<^bsub>ML\<^esub> v \<union> (\<Union>v \<in> set vs. fv\<^bsub>ML\<^esub> v)" |
-"fv\<^bsub>ML\<^esub> (Lam\<^bsub>ML\<^esub> v) = {X. Suc X : fv\<^bsub>ML\<^esub> v}" |
-"fv\<^bsub>ML\<^esub> (C\<^sub>U nm vs) = (\<Union>v \<in> set vs. fv\<^bsub>ML\<^esub> v)" |
-"fv\<^bsub>ML\<^esub> (V\<^sub>U nm vs) = (\<Union>v \<in> set vs. fv\<^bsub>ML\<^esub> v)" |
-"fv\<^bsub>ML\<^esub> (Clo f vs n) = fv\<^bsub>ML\<^esub> f \<union> (\<Union>v \<in> set vs. fv\<^bsub>ML\<^esub> v)" |
-"fv\<^bsub>ML\<^esub> (apply v w) = fv\<^bsub>ML\<^esub> v \<union> fv\<^bsub>ML\<^esub> w"
+fun fv_ML :: "ml \<Rightarrow> ml_vname set" ("fv\<^sub>M\<^sub>L") where
+"fv\<^sub>M\<^sub>L (C\<^sub>M\<^sub>L nm) = {}" |
+"fv\<^sub>M\<^sub>L (V\<^sub>M\<^sub>L X) = {X}"  |
+"fv\<^sub>M\<^sub>L (A\<^sub>M\<^sub>L v vs) = fv\<^sub>M\<^sub>L v \<union> (\<Union>v \<in> set vs. fv\<^sub>M\<^sub>L v)" |
+"fv\<^sub>M\<^sub>L (Lam\<^sub>M\<^sub>L v) = {X. Suc X : fv\<^sub>M\<^sub>L v}" |
+"fv\<^sub>M\<^sub>L (C\<^sub>U nm vs) = (\<Union>v \<in> set vs. fv\<^sub>M\<^sub>L v)" |
+"fv\<^sub>M\<^sub>L (V\<^sub>U nm vs) = (\<Union>v \<in> set vs. fv\<^sub>M\<^sub>L v)" |
+"fv\<^sub>M\<^sub>L (Clo f vs n) = fv\<^sub>M\<^sub>L f \<union> (\<Union>v \<in> set vs. fv\<^sub>M\<^sub>L v)" |
+"fv\<^sub>M\<^sub>L (apply v w) = fv\<^sub>M\<^sub>L v \<union> fv\<^sub>M\<^sub>L w"
 
 primrec fv :: "tm \<Rightarrow> vname set" where
 "fv (C nm) = {}" |
@@ -244,10 +244,10 @@ by(induct ts arbitrary:t) auto
 subsection "Lifting and Substitution"
 
 fun lift_ml :: "nat \<Rightarrow> ml \<Rightarrow> ml" ("lift") where
-"lift i (C\<^bsub>ML\<^esub> nm) = C\<^bsub>ML\<^esub> nm" |
-"lift i (V\<^bsub>ML\<^esub> X) = V\<^bsub>ML\<^esub> X" |
-"lift i (A\<^bsub>ML\<^esub> v vs) = A\<^bsub>ML\<^esub> (lift i v) (map (lift i) vs)" |
-"lift i (Lam\<^bsub>ML\<^esub> v) = Lam\<^bsub>ML\<^esub> (lift i v)" |
+"lift i (C\<^sub>M\<^sub>L nm) = C\<^sub>M\<^sub>L nm" |
+"lift i (V\<^sub>M\<^sub>L X) = V\<^sub>M\<^sub>L X" |
+"lift i (A\<^sub>M\<^sub>L v vs) = A\<^sub>M\<^sub>L (lift i v) (map (lift i) vs)" |
+"lift i (Lam\<^sub>M\<^sub>L v) = Lam\<^sub>M\<^sub>L (lift i v)" |
 "lift i (C\<^sub>U nm vs) = C\<^sub>U nm (map (lift i) vs)" |
 "lift i (V\<^sub>U x vs) = V\<^sub>U (if x < i then x else x+1) (map (lift i) vs)" |
 "lift i (Clo v vs n) = Clo (lift i v) (map (lift i) vs) n" |
@@ -262,15 +262,15 @@ fun lift_tm :: "nat \<Rightarrow> tm \<Rightarrow> tm" ("lift") where
 "lift i (\<Lambda> t) = \<Lambda>(lift (i+1) t)" |
 "lift i (term v) = term (lift i v)"
 
-fun lift_ML :: "nat \<Rightarrow> ml \<Rightarrow> ml" ("lift\<^bsub>ML\<^esub>") where
-"lift\<^bsub>ML\<^esub> i (C\<^bsub>ML\<^esub> nm) = C\<^bsub>ML\<^esub> nm" |
-"lift\<^bsub>ML\<^esub> i (V\<^bsub>ML\<^esub> X) = V\<^bsub>ML\<^esub> (if X < i then X else X+1)" |
-"lift\<^bsub>ML\<^esub> i (A\<^bsub>ML\<^esub> v vs) = A\<^bsub>ML\<^esub> (lift\<^bsub>ML\<^esub> i v) (map (lift\<^bsub>ML\<^esub> i) vs)" |
-"lift\<^bsub>ML\<^esub> i (Lam\<^bsub>ML\<^esub> v) = Lam\<^bsub>ML\<^esub> (lift\<^bsub>ML\<^esub> (i+1) v)" |
-"lift\<^bsub>ML\<^esub> i (C\<^sub>U nm vs) = C\<^sub>U nm (map (lift\<^bsub>ML\<^esub> i) vs)" |
-"lift\<^bsub>ML\<^esub> i (V\<^sub>U x vs) = V\<^sub>U x (map (lift\<^bsub>ML\<^esub> i) vs)" |
-"lift\<^bsub>ML\<^esub> i (Clo v vs n) = Clo (lift\<^bsub>ML\<^esub> i v) (map (lift\<^bsub>ML\<^esub> i) vs) n" |
-"lift\<^bsub>ML\<^esub> i (apply u v) = apply (lift\<^bsub>ML\<^esub> i u) (lift\<^bsub>ML\<^esub> i v)"
+fun lift_ML :: "nat \<Rightarrow> ml \<Rightarrow> ml" ("lift\<^sub>M\<^sub>L") where
+"lift\<^sub>M\<^sub>L i (C\<^sub>M\<^sub>L nm) = C\<^sub>M\<^sub>L nm" |
+"lift\<^sub>M\<^sub>L i (V\<^sub>M\<^sub>L X) = V\<^sub>M\<^sub>L (if X < i then X else X+1)" |
+"lift\<^sub>M\<^sub>L i (A\<^sub>M\<^sub>L v vs) = A\<^sub>M\<^sub>L (lift\<^sub>M\<^sub>L i v) (map (lift\<^sub>M\<^sub>L i) vs)" |
+"lift\<^sub>M\<^sub>L i (Lam\<^sub>M\<^sub>L v) = Lam\<^sub>M\<^sub>L (lift\<^sub>M\<^sub>L (i+1) v)" |
+"lift\<^sub>M\<^sub>L i (C\<^sub>U nm vs) = C\<^sub>U nm (map (lift\<^sub>M\<^sub>L i) vs)" |
+"lift\<^sub>M\<^sub>L i (V\<^sub>U x vs) = V\<^sub>U x (map (lift\<^sub>M\<^sub>L i) vs)" |
+"lift\<^sub>M\<^sub>L i (Clo v vs n) = Clo (lift\<^sub>M\<^sub>L i v) (map (lift\<^sub>M\<^sub>L i) vs) n" |
+"lift\<^sub>M\<^sub>L i (apply u v) = apply (lift\<^sub>M\<^sub>L i u) (lift\<^sub>M\<^sub>L i v)"
 
 definition
  cons :: "tm \<Rightarrow> (nat \<Rightarrow> tm) \<Rightarrow> (nat \<Rightarrow> tm)" (infix "##" 65) where
@@ -278,7 +278,7 @@ definition
 
 definition
  cons_ML :: "ml \<Rightarrow> (nat \<Rightarrow> ml) \<Rightarrow> (nat \<Rightarrow> ml)" (infix "##" 65) where
-"v##\<sigma> \<equiv> \<lambda>i. case i of 0 \<Rightarrow> v::ml | Suc j \<Rightarrow> lift\<^bsub>ML\<^esub> 0 (\<sigma> j)"
+"v##\<sigma> \<equiv> \<lambda>i. case i of 0 \<Rightarrow> v::ml | Suc j \<Rightarrow> lift\<^sub>M\<^sub>L 0 (\<sigma> j)"
 
 text{* Only for pure terms! *}
 primrec subst :: "(nat \<Rightarrow> tm) \<Rightarrow> tm \<Rightarrow> tm"
@@ -288,15 +288,15 @@ where
 | "subst \<sigma> (\<Lambda> t) = \<Lambda>(subst (V 0 ## \<sigma>) t)"
 | "subst \<sigma> (s\<bullet>t) = (subst \<sigma> s) \<bullet> (subst \<sigma> t)"
 
-fun subst_ML :: "(nat \<Rightarrow> ml) \<Rightarrow> ml \<Rightarrow> ml" ("subst\<^bsub>ML\<^esub>") where
-"subst\<^bsub>ML\<^esub> \<sigma> (C\<^bsub>ML\<^esub> nm) = C\<^bsub>ML\<^esub> nm" |
-"subst\<^bsub>ML\<^esub> \<sigma> (V\<^bsub>ML\<^esub> X) = \<sigma> X" |
-"subst\<^bsub>ML\<^esub> \<sigma> (A\<^bsub>ML\<^esub> v vs) = A\<^bsub>ML\<^esub> (subst\<^bsub>ML\<^esub> \<sigma> v) (map (subst\<^bsub>ML\<^esub> \<sigma>) vs)" |
-"subst\<^bsub>ML\<^esub> \<sigma> (Lam\<^bsub>ML\<^esub> v) = Lam\<^bsub>ML\<^esub> (subst\<^bsub>ML\<^esub> (V\<^bsub>ML\<^esub> 0 ## \<sigma>) v)" |
-"subst\<^bsub>ML\<^esub> \<sigma> (C\<^sub>U nm vs) = C\<^sub>U nm (map (subst\<^bsub>ML\<^esub> \<sigma>) vs)" |
-"subst\<^bsub>ML\<^esub> \<sigma> (V\<^sub>U x vs) = V\<^sub>U x (map (subst\<^bsub>ML\<^esub> \<sigma>) vs)" |
-"subst\<^bsub>ML\<^esub> \<sigma> (Clo v vs n) = Clo (subst\<^bsub>ML\<^esub> \<sigma> v) (map (subst\<^bsub>ML\<^esub> \<sigma>) vs) n" |
-"subst\<^bsub>ML\<^esub> \<sigma> (apply u v) = apply (subst\<^bsub>ML\<^esub> \<sigma> u) (subst\<^bsub>ML\<^esub> \<sigma> v)"
+fun subst_ML :: "(nat \<Rightarrow> ml) \<Rightarrow> ml \<Rightarrow> ml" ("subst\<^sub>M\<^sub>L") where
+"subst\<^sub>M\<^sub>L \<sigma> (C\<^sub>M\<^sub>L nm) = C\<^sub>M\<^sub>L nm" |
+"subst\<^sub>M\<^sub>L \<sigma> (V\<^sub>M\<^sub>L X) = \<sigma> X" |
+"subst\<^sub>M\<^sub>L \<sigma> (A\<^sub>M\<^sub>L v vs) = A\<^sub>M\<^sub>L (subst\<^sub>M\<^sub>L \<sigma> v) (map (subst\<^sub>M\<^sub>L \<sigma>) vs)" |
+"subst\<^sub>M\<^sub>L \<sigma> (Lam\<^sub>M\<^sub>L v) = Lam\<^sub>M\<^sub>L (subst\<^sub>M\<^sub>L (V\<^sub>M\<^sub>L 0 ## \<sigma>) v)" |
+"subst\<^sub>M\<^sub>L \<sigma> (C\<^sub>U nm vs) = C\<^sub>U nm (map (subst\<^sub>M\<^sub>L \<sigma>) vs)" |
+"subst\<^sub>M\<^sub>L \<sigma> (V\<^sub>U x vs) = V\<^sub>U x (map (subst\<^sub>M\<^sub>L \<sigma>) vs)" |
+"subst\<^sub>M\<^sub>L \<sigma> (Clo v vs n) = Clo (subst\<^sub>M\<^sub>L \<sigma> v) (map (subst\<^sub>M\<^sub>L \<sigma>) vs) n" |
+"subst\<^sub>M\<^sub>L \<sigma> (apply u v) = apply (subst\<^sub>M\<^sub>L \<sigma> u) (subst\<^sub>M\<^sub>L \<sigma> v)"
 (* FIXME currrently needed for code generator
 lemmas [code] = lift_tm.simps lift_ml.simps
 lemmas [code] = subst_ML.simps *)
@@ -306,20 +306,20 @@ abbreviation
   "subst_decr k t \<equiv> \<lambda>n. if n<k then V n else if n=k then t else V(n - 1)"
 abbreviation
   subst_decr_ML :: "nat \<Rightarrow> ml \<Rightarrow> nat \<Rightarrow> ml" where
-"subst_decr_ML k v \<equiv> \<lambda>n. if n<k then V\<^bsub>ML\<^esub> n else if n=k then v else V\<^bsub>ML\<^esub>(n - 1)"
+"subst_decr_ML k v \<equiv> \<lambda>n. if n<k then V\<^sub>M\<^sub>L n else if n=k then v else V\<^sub>M\<^sub>L(n - 1)"
 abbreviation
   subst1 :: "tm \<Rightarrow> tm \<Rightarrow> nat \<Rightarrow> tm" ("(_/[_'/_])" [300, 0, 0] 300) where
  "s[t/k] \<equiv> subst (subst_decr k t) s"
 abbreviation
   subst1_ML :: "ml \<Rightarrow> ml \<Rightarrow> nat \<Rightarrow> ml" ("(_/[_'/_])" [300, 0, 0] 300) where
- "u[v/k] \<equiv> subst\<^bsub>ML\<^esub> (subst_decr_ML k v) u"
+ "u[v/k] \<equiv> subst\<^sub>M\<^sub>L (subst_decr_ML k v) u"
 
 lemma apply_cons[simp]:
   "(t##\<sigma>) i = (if i=0 then t::tm else lift 0 (\<sigma>(i - 1)))"
 by(simp add: cons_def split:nat.split)
 
 lemma apply_cons_ML[simp]:
-  "(v##\<sigma>) i = (if i=0 then v::ml else lift\<^bsub>ML\<^esub> 0 (\<sigma>(i - 1)))"
+  "(v##\<sigma>) i = (if i=0 then v::ml else lift\<^sub>M\<^sub>L 0 (\<sigma>(i - 1)))"
 by(simp add: cons_ML_def split:nat.split)
 
 lemma lift_foldl_At[simp]:
@@ -335,17 +335,17 @@ lemma lift_lift_tm: fixes t :: tm shows
 by(induct t arbitrary: i rule:lift_tm.induct)(simp_all add:lift_lift_ml)
 
 lemma lift_lift_ML:
-  "i < k+1 \<Longrightarrow> lift\<^bsub>ML\<^esub> (Suc k) (lift\<^bsub>ML\<^esub> i v) = lift\<^bsub>ML\<^esub> i (lift\<^bsub>ML\<^esub> k v)"
+  "i < k+1 \<Longrightarrow> lift\<^sub>M\<^sub>L (Suc k) (lift\<^sub>M\<^sub>L i v) = lift\<^sub>M\<^sub>L i (lift\<^sub>M\<^sub>L k v)"
 by(induct v arbitrary: i rule:lift_ML.induct)
   simp_all
 
 lemma lift_lift_ML_comm:
-  "lift j (lift\<^bsub>ML\<^esub> i v) = lift\<^bsub>ML\<^esub> i (lift j v)"
+  "lift j (lift\<^sub>M\<^sub>L i v) = lift\<^sub>M\<^sub>L i (lift j v)"
 by(induct v arbitrary: i j rule:lift_ML.induct)
   simp_all
 
 lemma V_ML_cons_ML_subst_decr[simp]:
-  "V\<^bsub>ML\<^esub> 0 ## subst_decr_ML k v = subst_decr_ML (Suc k) (lift\<^bsub>ML\<^esub> 0 v)"
+  "V\<^sub>M\<^sub>L 0 ## subst_decr_ML k v = subst_decr_ML (Suc k) (lift\<^sub>M\<^sub>L 0 v)"
 by(rule ext)(simp add:cons_ML_def split:nat.split)
 
 lemma shift_subst_decr[simp]:
@@ -356,7 +356,7 @@ lemma lift_comp_subst_decr[simp]:
   "lift 0 o subst_decr_ML k v = subst_decr_ML k (lift 0 v)"
 by(rule ext) simp
 
-lemma subst_ML_ext: "\<forall>i. \<sigma> i = \<sigma>' i \<Longrightarrow> subst\<^bsub>ML\<^esub> \<sigma> v = subst\<^bsub>ML\<^esub> \<sigma>' v"
+lemma subst_ML_ext: "\<forall>i. \<sigma> i = \<sigma>' i \<Longrightarrow> subst\<^sub>M\<^sub>L \<sigma> v = subst\<^sub>M\<^sub>L \<sigma>' v"
 by(metis ext)
 
 lemma subst_ext: "\<forall>i. \<sigma> i = \<sigma>' i \<Longrightarrow> subst \<sigma> v = subst \<sigma>' v"
@@ -365,17 +365,17 @@ by(metis ext)
 lemma lift_Pure_tms[simp]: "pure t \<Longrightarrow> pure(lift k t)"
 by(induct arbitrary:k pred:pure) simp_all
 
-lemma cons_ML_V_ML[simp]: "(V\<^bsub>ML\<^esub> 0 ## V\<^bsub>ML\<^esub>) = V\<^bsub>ML\<^esub>"
+lemma cons_ML_V_ML[simp]: "(V\<^sub>M\<^sub>L 0 ## V\<^sub>M\<^sub>L) = V\<^sub>M\<^sub>L"
 by(rule ext) simp
 
 lemma cons_V[simp]: "(V 0 ## V) = V"
 by(rule ext) simp
 
-lemma lift_o_shift: "lift k \<circ> (V\<^bsub>ML\<^esub> 0 ## \<sigma>) = (V\<^bsub>ML\<^esub> 0 ## (lift k \<circ> \<sigma>))"
+lemma lift_o_shift: "lift k \<circ> (V\<^sub>M\<^sub>L 0 ## \<sigma>) = (V\<^sub>M\<^sub>L 0 ## (lift k \<circ> \<sigma>))"
 by(rule ext)(simp add: lift_lift_ML_comm)
 
 lemma lift_subst_ML:
- "lift k (subst\<^bsub>ML\<^esub> \<sigma> v) = subst\<^bsub>ML\<^esub> (lift k \<circ> \<sigma>) (lift k v)"
+ "lift k (subst\<^sub>M\<^sub>L \<sigma> v) = subst\<^sub>M\<^sub>L (lift k \<circ> \<sigma>) (lift k v)"
 apply(induct \<sigma> v rule:subst_ML.induct)
 apply(simp_all add: o_assoc lift_o_shift del:apply_cons_ML)
 apply(simp add:o_def)
@@ -389,30 +389,30 @@ apply(subst lift_lift_ML_comm)apply simp
 done
 
 lemma lift_ML_subst_ML:
- "lift\<^bsub>ML\<^esub> k (subst\<^bsub>ML\<^esub> \<sigma> v) =
-  subst\<^bsub>ML\<^esub> (\<lambda>i. if i<k then lift\<^bsub>ML\<^esub> k (\<sigma> i) else if i=k then V\<^bsub>ML\<^esub> k else lift\<^bsub>ML\<^esub> k (\<sigma>(i - 1))) (lift\<^bsub>ML\<^esub> k v)"
-  (is "_ = subst\<^bsub>ML\<^esub> (?insrt k \<sigma>) (lift\<^bsub>ML\<^esub> k v)")
+ "lift\<^sub>M\<^sub>L k (subst\<^sub>M\<^sub>L \<sigma> v) =
+  subst\<^sub>M\<^sub>L (\<lambda>i. if i<k then lift\<^sub>M\<^sub>L k (\<sigma> i) else if i=k then V\<^sub>M\<^sub>L k else lift\<^sub>M\<^sub>L k (\<sigma>(i - 1))) (lift\<^sub>M\<^sub>L k v)"
+  (is "_ = subst\<^sub>M\<^sub>L (?insrt k \<sigma>) (lift\<^sub>M\<^sub>L k v)")
 apply (induct k v arbitrary: \<sigma> k rule: lift_ML.induct)
 apply (simp_all add: o_assoc lift_o_shift)
-apply(subgoal_tac "V\<^bsub>ML\<^esub> 0 ## ?insrt k \<sigma> = ?insrt (Suc k) (V\<^bsub>ML\<^esub> 0 ## \<sigma>)")
+apply(subgoal_tac "V\<^sub>M\<^sub>L 0 ## ?insrt k \<sigma> = ?insrt (Suc k) (V\<^sub>M\<^sub>L 0 ## \<sigma>)")
  apply simp
 apply (simp add:fun_eq_iff lift_lift_ML cons_ML_def split:nat.split)
 done
 
 corollary subst_cons_lift:
- "subst\<^bsub>ML\<^esub> (V\<^bsub>ML\<^esub> 0 ## \<sigma>) o (lift\<^bsub>ML\<^esub> 0) = lift\<^bsub>ML\<^esub> 0 o (subst\<^bsub>ML\<^esub> \<sigma>)"
+ "subst\<^sub>M\<^sub>L (V\<^sub>M\<^sub>L 0 ## \<sigma>) o (lift\<^sub>M\<^sub>L 0) = lift\<^sub>M\<^sub>L 0 o (subst\<^sub>M\<^sub>L \<sigma>)"
 apply(rule ext)
 apply(simp add: lift_ML_subst_ML)
-apply(subgoal_tac "(V\<^bsub>ML\<^esub> 0 ## \<sigma>) = (\<lambda>i. if i = 0 then V\<^bsub>ML\<^esub> 0 else lift\<^bsub>ML\<^esub> 0 (\<sigma> (i - 1)))")
+apply(subgoal_tac "(V\<^sub>M\<^sub>L 0 ## \<sigma>) = (\<lambda>i. if i = 0 then V\<^sub>M\<^sub>L 0 else lift\<^sub>M\<^sub>L 0 (\<sigma> (i - 1)))")
  apply simp
 apply(rule ext, simp)
 done
 
-lemma lift_ML_id[simp]: "closed\<^bsub>ML\<^esub> k v \<Longrightarrow> lift\<^bsub>ML\<^esub> k v = v"
+lemma lift_ML_id[simp]: "closed\<^sub>M\<^sub>L k v \<Longrightarrow> lift\<^sub>M\<^sub>L k v = v"
 by(induct k v rule: lift_ML.induct)(simp_all add:list_eq_iff_nth_eq)
 
 lemma subst_ML_id:
-  "closed\<^bsub>ML\<^esub> k v \<Longrightarrow> \<forall>i<k. \<sigma> i = V\<^bsub>ML\<^esub> i \<Longrightarrow> subst\<^bsub>ML\<^esub> \<sigma> v = v"
+  "closed\<^sub>M\<^sub>L k v \<Longrightarrow> \<forall>i<k. \<sigma> i = V\<^sub>M\<^sub>L i \<Longrightarrow> subst\<^sub>M\<^sub>L \<sigma> v = v"
 apply (induct \<sigma> v arbitrary: k rule: subst_ML.induct)
 apply (auto simp add: list_eq_iff_nth_eq)
    apply(simp add:Ball_def)
@@ -432,15 +432,15 @@ apply(erule_tac x="k" in meta_allE)
 apply simp
 done
 
-corollary subst_ML_id2[simp]: "closed\<^bsub>ML\<^esub> 0 v \<Longrightarrow> subst\<^bsub>ML\<^esub> \<sigma> v = v"
+corollary subst_ML_id2[simp]: "closed\<^sub>M\<^sub>L 0 v \<Longrightarrow> subst\<^sub>M\<^sub>L \<sigma> v = v"
 using subst_ML_id[where k=0] by simp
 
 lemma subst_ML_coincidence:
-  "closed\<^bsub>ML\<^esub> k v \<Longrightarrow> \<forall>i<k. \<sigma> i = \<sigma>' i \<Longrightarrow> subst\<^bsub>ML\<^esub> \<sigma> v = subst\<^bsub>ML\<^esub> \<sigma>' v"
+  "closed\<^sub>M\<^sub>L k v \<Longrightarrow> \<forall>i<k. \<sigma> i = \<sigma>' i \<Longrightarrow> subst\<^sub>M\<^sub>L \<sigma> v = subst\<^sub>M\<^sub>L \<sigma>' v"
 by (induct \<sigma> v arbitrary: k \<sigma>' rule: subst_ML.induct) auto
 
 lemma subst_ML_comp:
-  "subst\<^bsub>ML\<^esub> \<sigma> (subst\<^bsub>ML\<^esub> \<sigma>' v) = subst\<^bsub>ML\<^esub> (subst\<^bsub>ML\<^esub> \<sigma>  \<circ> \<sigma>') v"
+  "subst\<^sub>M\<^sub>L \<sigma> (subst\<^sub>M\<^sub>L \<sigma>' v) = subst\<^sub>M\<^sub>L (subst\<^sub>M\<^sub>L \<sigma>  \<circ> \<sigma>') v"
 apply (induct \<sigma>' v arbitrary: \<sigma> rule: subst_ML.induct)
 apply (simp_all add: list_eq_iff_nth_eq)
 apply(rule subst_ML_ext)
@@ -449,27 +449,27 @@ apply (metis o_apply subst_cons_lift)
 done
 
 lemma subst_ML_comp2:
-  "\<forall>i. \<sigma>'' i = subst\<^bsub>ML\<^esub> \<sigma> (\<sigma>' i) \<Longrightarrow> subst\<^bsub>ML\<^esub> \<sigma> (subst\<^bsub>ML\<^esub> \<sigma>' v) = subst\<^bsub>ML\<^esub> \<sigma>'' v"
+  "\<forall>i. \<sigma>'' i = subst\<^sub>M\<^sub>L \<sigma> (\<sigma>' i) \<Longrightarrow> subst\<^sub>M\<^sub>L \<sigma> (subst\<^sub>M\<^sub>L \<sigma>' v) = subst\<^sub>M\<^sub>L \<sigma>'' v"
 by(simp add:subst_ML_comp subst_ML_ext)
 
 lemma closed_tm_ML_foldl_At:
-  "closed\<^bsub>ML\<^esub> k (t \<bullet>\<bullet> ts) \<longleftrightarrow> closed\<^bsub>ML\<^esub> k t \<and> (\<forall>t \<in> set ts. closed\<^bsub>ML\<^esub> k t)"
+  "closed\<^sub>M\<^sub>L k (t \<bullet>\<bullet> ts) \<longleftrightarrow> closed\<^sub>M\<^sub>L k t \<and> (\<forall>t \<in> set ts. closed\<^sub>M\<^sub>L k t)"
 by(induct ts arbitrary: t) simp_all
 
 lemma closed_ML_lift[simp]:
-  fixes v :: ml shows "closed\<^bsub>ML\<^esub> k v \<Longrightarrow> closed\<^bsub>ML\<^esub> k (lift m v)"
+  fixes v :: ml shows "closed\<^sub>M\<^sub>L k v \<Longrightarrow> closed\<^sub>M\<^sub>L k (lift m v)"
 by(induct k v arbitrary: m rule: lift_ML.induct)
   (simp_all add:list_eq_iff_nth_eq)
 
-lemma closed_ML_Suc: "closed\<^bsub>ML\<^esub> n v \<Longrightarrow> closed\<^bsub>ML\<^esub> (Suc n) (lift\<^bsub>ML\<^esub> k v)"
+lemma closed_ML_Suc: "closed\<^sub>M\<^sub>L n v \<Longrightarrow> closed\<^sub>M\<^sub>L (Suc n) (lift\<^sub>M\<^sub>L k v)"
 by (induct k v arbitrary: n rule: lift_ML.induct) simp_all
 
 lemma closed_ML_subst_ML:
-  "\<forall>i. closed\<^bsub>ML\<^esub> k (\<sigma> i) \<Longrightarrow> closed\<^bsub>ML\<^esub> k (subst\<^bsub>ML\<^esub> \<sigma> v)"
+  "\<forall>i. closed\<^sub>M\<^sub>L k (\<sigma> i) \<Longrightarrow> closed\<^sub>M\<^sub>L k (subst\<^sub>M\<^sub>L \<sigma> v)"
 by(induct \<sigma> v arbitrary: k rule: subst_ML.induct) (auto simp: closed_ML_Suc)
 
 lemma closed_ML_subst_ML2:
-  "closed\<^bsub>ML\<^esub> k v \<Longrightarrow> \<forall>i<k. closed\<^bsub>ML\<^esub> l (\<sigma> i) \<Longrightarrow> closed\<^bsub>ML\<^esub> l (subst\<^bsub>ML\<^esub> \<sigma> v)"
+  "closed\<^sub>M\<^sub>L k v \<Longrightarrow> \<forall>i<k. closed\<^sub>M\<^sub>L l (\<sigma> i) \<Longrightarrow> closed\<^sub>M\<^sub>L l (subst\<^sub>M\<^sub>L \<sigma> v)"
 by(induct \<sigma> v arbitrary: k l rule: subst_ML.induct)(auto simp: closed_ML_Suc)
 
 
@@ -654,11 +654,11 @@ done
 
 declare conj_cong[fundef_cong]
 
-function no_match_ML ("no'_match\<^bsub>ML\<^esub>") where
-"no_match\<^bsub>ML\<^esub> ps os =
+function no_match_ML ("no'_match\<^sub>M\<^sub>L") where
+"no_match\<^sub>M\<^sub>L ps os =
   (\<exists>i < min (size os) (size ps).
    \<exists>nm nm' vs vs'. (rev ps)!i = C\<^sub>U nm vs \<and> (rev os)!i = C\<^sub>U nm' vs' \<and>
-      (nm=nm' \<longrightarrow> no_match\<^bsub>ML\<^esub> vs vs'))"
+      (nm=nm' \<longrightarrow> no_match\<^sub>M\<^sub>L vs vs'))"
 by pat_completeness auto
 termination
 apply(relation "measure(%(vs::ml list,_). \<Sum>v\<leftarrow>vs. size v)")
@@ -668,7 +668,7 @@ done
 
 abbreviation
 "no_match_compR nm os \<equiv>
-  \<forall>(nm',ps,v)\<in> compR. nm=nm' \<longrightarrow> no_match\<^bsub>ML\<^esub> ps os"
+  \<forall>(nm',ps,v)\<in> compR. nm=nm' \<longrightarrow> no_match\<^sub>M\<^sub>L ps os"
 
 declare no_match_ML.simps[simp del]
 
@@ -683,17 +683,17 @@ where
 | "ss \<Rightarrow> ts \<equiv> (ss, ts) \<in> Red_ml_list"
 | "s \<Rightarrow>* t \<equiv> (s, t) \<in> Red_ml^*"
  -- {* ML $\beta$-reduction *}
-| "A\<^bsub>ML\<^esub> (Lam\<^bsub>ML\<^esub> u) [v] \<Rightarrow> u[v/0]"
+| "A\<^sub>M\<^sub>L (Lam\<^sub>M\<^sub>L u) [v] \<Rightarrow> u[v/0]"
  -- "Execution of a compiled rewrite rule"
-| "(nm,vs,v) : compR \<Longrightarrow> \<forall> i. closed\<^bsub>ML\<^esub> 0 (\<sigma> i) \<Longrightarrow>
-   A\<^bsub>ML\<^esub> (C\<^bsub>ML\<^esub> nm) (map (subst\<^bsub>ML\<^esub> \<sigma>) vs) \<Rightarrow> subst\<^bsub>ML\<^esub> \<sigma> v"
+| "(nm,vs,v) : compR \<Longrightarrow> \<forall> i. closed\<^sub>M\<^sub>L 0 (\<sigma> i) \<Longrightarrow>
+   A\<^sub>M\<^sub>L (C\<^sub>M\<^sub>L nm) (map (subst\<^sub>M\<^sub>L \<sigma>) vs) \<Rightarrow> subst\<^sub>M\<^sub>L \<sigma> v"
 -- {* default rule: *}
-| "\<forall>i. closed\<^bsub>ML\<^esub> 0 (\<sigma> i)
-   \<Longrightarrow> vs = map V\<^bsub>ML\<^esub> [0..<arity nm] \<Longrightarrow> vs' = map (subst\<^bsub>ML\<^esub> \<sigma>) vs
+| "\<forall>i. closed\<^sub>M\<^sub>L 0 (\<sigma> i)
+   \<Longrightarrow> vs = map V\<^sub>M\<^sub>L [0..<arity nm] \<Longrightarrow> vs' = map (subst\<^sub>M\<^sub>L \<sigma>) vs
    \<Longrightarrow> no_match_compR nm vs'
-   \<Longrightarrow> A\<^bsub>ML\<^esub> (C\<^bsub>ML\<^esub> nm) vs' \<Rightarrow> subst\<^bsub>ML\<^esub> \<sigma> (C\<^sub>U nm vs)"
+   \<Longrightarrow> A\<^sub>M\<^sub>L (C\<^sub>M\<^sub>L nm) vs' \<Rightarrow> subst\<^sub>M\<^sub>L \<sigma> (C\<^sub>U nm vs)"
  -- {* Equations for function \texttt{apply}*}
-| apply_Clo1: "apply (Clo f vs (Suc 0)) v \<Rightarrow> A\<^bsub>ML\<^esub> f (v # vs)"
+| apply_Clo1: "apply (Clo f vs (Suc 0)) v \<Rightarrow> A\<^sub>M\<^sub>L f (v # vs)"
 | apply_Clo2: "n > 0 \<Longrightarrow>
  apply (Clo f vs (Suc n)) v \<Rightarrow> Clo f (v # vs) n"
 | apply_C: "apply (C\<^sub>U nm vs) v \<Rightarrow> C\<^sub>U nm (v # vs)"
@@ -705,8 +705,8 @@ where
 | ctxt_Clo3: "vs \<Rightarrow> vs' \<Longrightarrow> Clo f vs n \<Rightarrow> Clo f vs' n"
 | ctxt_apply1: "s \<Rightarrow> s'   \<Longrightarrow> apply s t \<Rightarrow> apply s' t"
 | ctxt_apply2: "t \<Rightarrow> t'   \<Longrightarrow> apply s t \<Rightarrow> apply s t'"
-| ctxt_A_ML1: "f \<Rightarrow> f'   \<Longrightarrow> A\<^bsub>ML\<^esub> f vs \<Rightarrow> A\<^bsub>ML\<^esub> f' vs"
-| ctxt_A_ML2: "vs \<Rightarrow> vs' \<Longrightarrow> A\<^bsub>ML\<^esub> f vs \<Rightarrow> A\<^bsub>ML\<^esub> f vs'"
+| ctxt_A_ML1: "f \<Rightarrow> f'   \<Longrightarrow> A\<^sub>M\<^sub>L f vs \<Rightarrow> A\<^sub>M\<^sub>L f' vs"
+| ctxt_A_ML2: "vs \<Rightarrow> vs' \<Longrightarrow> A\<^sub>M\<^sub>L f vs \<Rightarrow> A\<^sub>M\<^sub>L f vs'"
 | ctxt_list1: "v \<Rightarrow> v'   \<Longrightarrow> v#vs \<Rightarrow> v'#vs"
 | ctxt_list2: "vs \<Rightarrow> vs' \<Longrightarrow> v#vs \<Rightarrow> v#vs'"
 
@@ -734,10 +734,10 @@ text{* First a special size function and some lemmas for the
 termination proof of the kernel function. *}
 
 fun size' :: "ml \<Rightarrow> nat" where
-"size' (C\<^bsub>ML\<^esub> nm) = 1" |
-"size' (V\<^bsub>ML\<^esub> X) = 1"  |
-"size' (A\<^bsub>ML\<^esub> v vs) = (size' v + (\<Sum>v\<leftarrow>vs. size' v))+1" |
-"size' (Lam\<^bsub>ML\<^esub> v) = size' v + 1" |
+"size' (C\<^sub>M\<^sub>L nm) = 1" |
+"size' (V\<^sub>M\<^sub>L X) = 1"  |
+"size' (A\<^sub>M\<^sub>L v vs) = (size' v + (\<Sum>v\<leftarrow>vs. size' v))+1" |
+"size' (Lam\<^sub>M\<^sub>L v) = size' v + 1" |
 "size' (C\<^sub>U nm vs) = (\<Sum>v\<leftarrow>vs. size' v)+1" |
 "size' (V\<^sub>U nm vs) = (\<Sum>v\<leftarrow>vs. size' v)+1" |
 "size' (Clo f vs n) = (size' f + (\<Sum>v\<leftarrow>vs. size' v))+1" |
@@ -751,7 +751,7 @@ corollary cor_listsum_size'[simp]:
  "v \<in> set vs \<Longrightarrow> size' v < Suc(m + listsum (map size' vs))"
 using listsum_size'[of v vs] by arith
 
-lemma size'_lift_ML: "size' (lift\<^bsub>ML\<^esub> k v) = size' v"
+lemma size'_lift_ML: "size' (lift\<^sub>M\<^sub>L k v) = size' v"
 apply(induct v arbitrary:k rule:size'.induct)
 apply simp_all
    apply(rule arg_cong[where f = listsum])
@@ -769,7 +769,7 @@ apply simp
 done
 
 lemma size'_subst_ML[simp]:
- "\<forall>i j. size'(\<sigma> i) = 1 \<Longrightarrow> size' (subst\<^bsub>ML\<^esub> \<sigma> v) = size' v"
+ "\<forall>i j. size'(\<sigma> i) = 1 \<Longrightarrow> size' (subst\<^sub>M\<^sub>L \<sigma> v) = size' v"
 apply(induct v arbitrary:\<sigma> rule:size'.induct)
 apply simp_all
     apply(rule arg_cong[where f = listsum])
@@ -807,14 +807,14 @@ apply simp
 done
 
 function kernel  :: "ml \<Rightarrow> tm"  ("_!" 300) where
-"(C\<^bsub>ML\<^esub> nm)! = C nm" |
-"(A\<^bsub>ML\<^esub> v vs)! = v! \<bullet>\<bullet> (map kernel (rev vs))" |
-"(Lam\<^bsub>ML\<^esub> v)! = \<Lambda> (((lift 0 v)[V\<^sub>U 0 []/0])!)" |
+"(C\<^sub>M\<^sub>L nm)! = C nm" |
+"(A\<^sub>M\<^sub>L v vs)! = v! \<bullet>\<bullet> (map kernel (rev vs))" |
+"(Lam\<^sub>M\<^sub>L v)! = \<Lambda> (((lift 0 v)[V\<^sub>U 0 []/0])!)" |
 "(C\<^sub>U nm vs)! = (C nm) \<bullet>\<bullet> (map kernel (rev vs))" |
 "(V\<^sub>U x vs)! = (V x) \<bullet>\<bullet> (map kernel (rev vs))" |
 "(Clo f vs n)! = f! \<bullet>\<bullet> (map kernel (rev vs))" |
 "(apply v w)! = v! \<bullet> (w!)" |
-"(V\<^bsub>ML\<^esub> X)! = undefined"
+"(V\<^sub>M\<^sub>L X)! = undefined"
 by pat_completeness auto
 termination by(relation "measure size'") auto
 
@@ -845,24 +845,24 @@ lemma pure_foldl:
  pure(foldl f t ts)"
 by(induct ts arbitrary: t) simp_all
 
-lemma pure_kernel: fixes v :: ml shows "closed\<^bsub>ML\<^esub> 0 v \<Longrightarrow> pure(v!)"
+lemma pure_kernel: fixes v :: ml shows "closed\<^sub>M\<^sub>L 0 v \<Longrightarrow> pure(v!)"
 proof(induct v rule:kernel.induct)
   case (3 v)
-  hence "closed\<^bsub>ML\<^esub> (Suc 0) (lift 0 v)" by simp
-  then have "subst\<^bsub>ML\<^esub> (\<lambda>n. V\<^sub>U 0 []) (lift 0 v) = lift 0 v[V\<^sub>U 0 []/0]"
+  hence "closed\<^sub>M\<^sub>L (Suc 0) (lift 0 v)" by simp
+  then have "subst\<^sub>M\<^sub>L (\<lambda>n. V\<^sub>U 0 []) (lift 0 v) = lift 0 v[V\<^sub>U 0 []/0]"
     by(rule subst_ML_coincidence) simp
-  moreover have "closed\<^bsub>ML\<^esub> 0 (subst\<^bsub>ML\<^esub> (\<lambda>n. V\<^sub>U 0 []) (lift 0 v))"
+  moreover have "closed\<^sub>M\<^sub>L 0 (subst\<^sub>M\<^sub>L (\<lambda>n. V\<^sub>U 0 []) (lift 0 v))"
     by(simp add: closed_ML_subst_ML)
-  ultimately have "closed\<^bsub>ML\<^esub> 0 (lift 0 v[V\<^sub>U 0 []/0])" by simp
+  ultimately have "closed\<^sub>M\<^sub>L 0 (lift 0 v[V\<^sub>U 0 []/0])" by simp
   thus ?case using 3(1) by (simp add:pure_foldl)
 qed (simp_all add:pure_foldl)
 
 corollary subst_V_kernel: fixes v :: ml shows
-  "closed\<^bsub>ML\<^esub> 0 v \<Longrightarrow> subst V (v!) = v!"
+  "closed\<^sub>M\<^sub>L 0 v \<Longrightarrow> subst V (v!) = v!"
 by (metis pure_kernel subst_V)
 
 lemma kernel_lift_tm: fixes v :: ml shows
-  "closed\<^bsub>ML\<^esub> 0 v \<Longrightarrow> (lift i v)! = lift i (v!)"
+  "closed\<^sub>M\<^sub>L 0 v \<Longrightarrow> (lift i v)! = lift i (v!)"
 apply(induct v arbitrary: i rule: kernel.induct)
 apply (simp_all add:list_eq_iff_nth_eq)
  apply(simp add: rev_nth)
@@ -874,7 +874,7 @@ apply(erule_tac x="Suc i" in meta_allE)
 apply(erule meta_impE)
 defer
 apply (simp add:lift_subst_ML)
-apply(subgoal_tac "lift (Suc i) \<circ> (\<lambda>n. if n = 0 then V\<^sub>U 0 [] else V\<^bsub>ML\<^esub> (n - 1)) = (\<lambda>n. if n = 0 then V\<^sub>U 0 [] else V\<^bsub>ML\<^esub> (n - 1))")
+apply(subgoal_tac "lift (Suc i) \<circ> (\<lambda>n. if n = 0 then V\<^sub>U 0 [] else V\<^sub>M\<^sub>L (n - 1)) = (\<lambda>n. if n = 0 then V\<^sub>U 0 [] else V\<^sub>M\<^sub>L (n - 1))")
 apply (simp add:lift_lift_ml)
 apply(rule ext)
 apply(simp)
@@ -890,26 +890,26 @@ text{* This function is only introduced to prove the involved susbtitution
 lemma @{text kernel_subst1} below. *}
 
 fun subst_ml :: "(nat \<Rightarrow> nat) \<Rightarrow> ml \<Rightarrow> ml" where
-"subst_ml \<sigma> (C\<^bsub>ML\<^esub> nm) = C\<^bsub>ML\<^esub> nm" |
-"subst_ml \<sigma> (V\<^bsub>ML\<^esub> X) = V\<^bsub>ML\<^esub> X" |
-"subst_ml \<sigma> (A\<^bsub>ML\<^esub> v vs) = A\<^bsub>ML\<^esub> (subst_ml \<sigma> v) (map (subst_ml \<sigma>) vs)" |
-"subst_ml \<sigma> (Lam\<^bsub>ML\<^esub> v) = Lam\<^bsub>ML\<^esub> (subst_ml \<sigma> v)" |
+"subst_ml \<sigma> (C\<^sub>M\<^sub>L nm) = C\<^sub>M\<^sub>L nm" |
+"subst_ml \<sigma> (V\<^sub>M\<^sub>L X) = V\<^sub>M\<^sub>L X" |
+"subst_ml \<sigma> (A\<^sub>M\<^sub>L v vs) = A\<^sub>M\<^sub>L (subst_ml \<sigma> v) (map (subst_ml \<sigma>) vs)" |
+"subst_ml \<sigma> (Lam\<^sub>M\<^sub>L v) = Lam\<^sub>M\<^sub>L (subst_ml \<sigma> v)" |
 "subst_ml \<sigma> (C\<^sub>U nm vs) = C\<^sub>U nm (map (subst_ml \<sigma>) vs)" |
 "subst_ml \<sigma> (V\<^sub>U x vs) = V\<^sub>U (\<sigma> x) (map (subst_ml \<sigma>) vs)" |
 "subst_ml \<sigma> (Clo v vs n) = Clo (subst_ml \<sigma> v) (map (subst_ml \<sigma>) vs) n" |
 "subst_ml \<sigma> (apply u v) = apply (subst_ml \<sigma> u) (subst_ml \<sigma> v)"
 
 lemma lift_ML_subst_ml:
-  "lift\<^bsub>ML\<^esub> k (subst_ml \<sigma> v) = subst_ml \<sigma> (lift\<^bsub>ML\<^esub> k v)"
+  "lift\<^sub>M\<^sub>L k (subst_ml \<sigma> v) = subst_ml \<sigma> (lift\<^sub>M\<^sub>L k v)"
 apply (induct \<sigma> v arbitrary: k rule:subst_ml.induct)
 apply (simp_all add:list_eq_iff_nth_eq)
 done
 
 lemma subst_ml_subst_ML:
-  "subst_ml \<sigma> (subst\<^bsub>ML\<^esub> \<sigma>' v) = subst\<^bsub>ML\<^esub> (subst_ml \<sigma> o \<sigma>') (subst_ml \<sigma> v)"
+  "subst_ml \<sigma> (subst\<^sub>M\<^sub>L \<sigma>' v) = subst\<^sub>M\<^sub>L (subst_ml \<sigma> o \<sigma>') (subst_ml \<sigma> v)"
 apply (induct \<sigma>' v arbitrary: \<sigma> rule: subst_ML.induct)
 apply(simp_all add:list_eq_iff_nth_eq)
-apply(subgoal_tac "(subst_ml \<sigma>' \<circ> V\<^bsub>ML\<^esub> 0 ## \<sigma>) = V\<^bsub>ML\<^esub> 0 ## (subst_ml \<sigma>' \<circ> \<sigma>)")
+apply(subgoal_tac "(subst_ml \<sigma>' \<circ> V\<^sub>M\<^sub>L 0 ## \<sigma>) = V\<^sub>M\<^sub>L 0 ## (subst_ml \<sigma>' \<circ> \<sigma>)")
 apply simp
 apply(rule ext)
 apply(simp add: lift_ML_subst_ml)
@@ -924,7 +924,7 @@ lemma subst_ml_comp:  "subst_ml \<sigma> (subst_ml \<sigma>' v) = subst_ml (\<si
 by(induct \<sigma>' v rule:subst_ml.induct)(simp_all add:list_eq_iff_nth_eq)
 
 lemma subst_kernel:
-  "closed\<^bsub>ML\<^esub> 0 v \<Longrightarrow>  subst (\<lambda>n. V(\<sigma> n)) (v!) = (subst_ml \<sigma> v)!"
+  "closed\<^sub>M\<^sub>L 0 v \<Longrightarrow>  subst (\<lambda>n. V(\<sigma> n)) (v!) = (subst_ml \<sigma> v)!"
 apply (induct v arbitrary: \<sigma> rule:kernel.induct)
 apply (simp_all add:list_eq_iff_nth_eq)
  apply(simp add: rev_nth)
@@ -946,8 +946,8 @@ apply(rule arg_cong[where f = kernel])
 apply(subgoal_tac "(nat_case 0 (\<lambda>k. Suc (\<sigma> k)) \<circ> Suc) = Suc o \<sigma>")
 prefer 2 apply(simp add:fun_eq_iff split:nat.split)
 apply(subgoal_tac "(subst_ml (nat_case 0 (\<lambda>k. Suc (\<sigma> k))) \<circ>
-               (\<lambda>n. if n = 0 then V\<^sub>U 0 [] else V\<^bsub>ML\<^esub> (n - 1)))
-             = (\<lambda>n. if n = 0 then V\<^sub>U 0 [] else V\<^bsub>ML\<^esub> (n - 1))")
+               (\<lambda>n. if n = 0 then V\<^sub>U 0 [] else V\<^sub>M\<^sub>L (n - 1)))
+             = (\<lambda>n. if n = 0 then V\<^sub>U 0 [] else V\<^sub>M\<^sub>L (n - 1))")
 apply simp
 apply(simp add: fun_eq_iff)
 done
@@ -956,18 +956,18 @@ lemma if_cong0: "If x y z = If x y z"
 by simp
 
 lemma kernel_subst1:
-  "closed\<^bsub>ML\<^esub> 0 v \<Longrightarrow> closed\<^bsub>ML\<^esub> (Suc 0) u \<Longrightarrow>
+  "closed\<^sub>M\<^sub>L 0 v \<Longrightarrow> closed\<^sub>M\<^sub>L (Suc 0) u \<Longrightarrow>
    kernel(u[v/0]) = (kernel((lift 0 u)[V\<^sub>U 0 []/0]))[v!/0]"
 proof(induct u arbitrary:v rule:kernel.induct)
   case (3 w)
   show ?case (is "?L = ?R")
   proof -
-    have "?L = \<Lambda>(lift 0 (w[lift\<^bsub>ML\<^esub> 0 v/Suc 0])[V\<^sub>U 0 []/0] !)"
+    have "?L = \<Lambda>(lift 0 (w[lift\<^sub>M\<^sub>L 0 v/Suc 0])[V\<^sub>U 0 []/0] !)"
       by (simp cong:if_cong0)
-    also have "\<dots> = \<Lambda>((lift 0 w)[lift\<^bsub>ML\<^esub> 0 (lift 0 v)/Suc 0][V\<^sub>U 0 []/0]!)"
+    also have "\<dots> = \<Lambda>((lift 0 w)[lift\<^sub>M\<^sub>L 0 (lift 0 v)/Suc 0][V\<^sub>U 0 []/0]!)"
       by(simp only: lift_subst_ML1 lift_lift_ML_comm)
-    also have "\<dots> = \<Lambda>(subst\<^bsub>ML\<^esub> (\<lambda>n. if n=0 then V\<^sub>U 0 [] else
-            if n=Suc 0 then lift 0 v else V\<^bsub>ML\<^esub> (n - 2)) (lift 0 w) !)"
+    also have "\<dots> = \<Lambda>(subst\<^sub>M\<^sub>L (\<lambda>n. if n=0 then V\<^sub>U 0 [] else
+            if n=Suc 0 then lift 0 v else V\<^sub>M\<^sub>L (n - 2)) (lift 0 w) !)"
       apply simp
       apply(rule arg_cong[where f = kernel])
       apply(rule subst_ML_comp2)
@@ -985,11 +985,11 @@ proof(induct u arbitrary:v rule:kernel.induct)
       apply(rule arg_cong[where f = \<Lambda>])
       apply(rule 3(1))
       apply (metis closed_ML_lift 3(2))
-      apply(subgoal_tac "closed\<^bsub>ML\<^esub> (Suc(Suc 0)) w")
+      apply(subgoal_tac "closed\<^sub>M\<^sub>L (Suc(Suc 0)) w")
       defer
       using 3
       apply force
-      apply(subgoal_tac  "closed\<^bsub>ML\<^esub> (Suc (Suc 0)) (lift 0 w)")
+      apply(subgoal_tac  "closed\<^sub>M\<^sub>L (Suc (Suc 0)) (lift 0 w)")
       defer
       apply(erule closed_ML_lift)
       apply(erule closed_ML_subst_ML2)
@@ -1005,7 +1005,7 @@ proof(induct u arbitrary:v rule:kernel.induct)
     finally have "?L = ?M" .
     have "?R = \<Lambda> (subst (V 0 ## subst_decr 0 (v!))
           (lift 0 (lift_ml 0 w[V\<^sub>U 0 []/Suc 0])[V\<^sub>U 0 []/0]!))"
-      apply(subgoal_tac "(V\<^bsub>ML\<^esub> 0 ## (\<lambda>n. if n = 0 then V\<^sub>U 0 [] else V\<^bsub>ML\<^esub> (n - Suc 0))) = subst_decr_ML (Suc 0) (V\<^sub>U 0 [])")
+      apply(subgoal_tac "(V\<^sub>M\<^sub>L 0 ## (\<lambda>n. if n = 0 then V\<^sub>U 0 [] else V\<^sub>M\<^sub>L (n - Suc 0))) = subst_decr_ML (Suc 0) (V\<^sub>U 0 [])")
       apply(simp cong:if_cong)
       apply(simp add:fun_eq_iff cons_ML_def split:nat.splits)
       done
@@ -1019,8 +1019,8 @@ proof(induct u arbitrary:v rule:kernel.induct)
     also have "(lift_ml 0 (lift_ml 0 w))[V\<^sub>U 1 []/Suc 0][V\<^sub>U 0 []/0] =
                (lift 0 (lift_ml 0 w))[V\<^sub>U 0 []/0][V\<^sub>U 1 []/ 0]" (is "?l = ?r")
     proof -
-      have "?l = subst\<^bsub>ML\<^esub> (\<lambda>n. if n= 0 then V\<^sub>U 0 [] else if n = 1 then V\<^sub>U 1 [] else
-                      V\<^bsub>ML\<^esub> (n - 2))
+      have "?l = subst\<^sub>M\<^sub>L (\<lambda>n. if n= 0 then V\<^sub>U 0 [] else if n = 1 then V\<^sub>U 1 [] else
+                      V\<^sub>M\<^sub>L (n - 2))
                (lift_ml 0 (lift_ml 0 w))"
       by(auto intro!:subst_ML_comp2)
     also have "\<dots> = ?r" by(auto intro!:subst_ML_comp2[symmetric])
@@ -1100,13 +1100,13 @@ primrec compile :: "tm \<Rightarrow> (nat \<Rightarrow> ml) \<Rightarrow> ml"
 where
   "compile (V x) \<sigma> = \<sigma> x"
 | "compile (C nm) \<sigma> =
-    (if arity nm > 0 then Clo (C\<^bsub>ML\<^esub> nm) [] (arity nm) else A\<^bsub>ML\<^esub> (C\<^bsub>ML\<^esub> nm) [])"
+    (if arity nm > 0 then Clo (C\<^sub>M\<^sub>L nm) [] (arity nm) else A\<^sub>M\<^sub>L (C\<^sub>M\<^sub>L nm) [])"
 | "compile (s \<bullet> t) \<sigma> = apply (compile s \<sigma>) (compile t \<sigma>)"
-| "compile (\<Lambda> t) \<sigma> = Clo (Lam\<^bsub>ML\<^esub> (compile t (V\<^bsub>ML\<^esub> 0 ## \<sigma>))) [] 1"
+| "compile (\<Lambda> t) \<sigma> = Clo (Lam\<^sub>M\<^sub>L (compile t (V\<^sub>M\<^sub>L 0 ## \<sigma>))) [] 1"
 
 text{* Compiler for open terms and for terms with fixed free variables: *}
 
-definition "comp_open t = compile t V\<^bsub>ML\<^esub>"
+definition "comp_open t = compile t V\<^sub>M\<^sub>L"
 abbreviation "comp_fixed t \<equiv> compile t (\<lambda>i. V\<^sub>U i [])"
 
 text{* Compiled rules: *}
@@ -1118,11 +1118,11 @@ fun comp_pat where
 "comp_pat t =
    (case head_tm t of
      C nm \<Rightarrow> C\<^sub>U nm (map comp_pat (rev (args_tm t)))
-   | V X \<Rightarrow> V\<^bsub>ML\<^esub> X)"
+   | V X \<Rightarrow> V\<^sub>M\<^sub>L X)"
 
 declare comp_pat.simps[simp del] size_args_less_size_tm[simp del]
 
-lemma comp_pat_V[simp]: "comp_pat(V X) = V\<^bsub>ML\<^esub> X"
+lemma comp_pat_V[simp]: "comp_pat(V X) = V\<^sub>M\<^sub>L X"
 by(simp add:comp_pat.simps)
 
 lemma comp_pat_C[simp]:
@@ -1137,15 +1137,15 @@ defs compR_def:
  "compR \<equiv> (\<lambda>(nm,ts,t). (nm, map comp_pat (rev ts), comp_open t)) ` R"
 
 
-lemma fv_ML_comp_open: "pure t \<Longrightarrow> fv\<^bsub>ML\<^esub>(comp_open t) = fv t"
+lemma fv_ML_comp_open: "pure t \<Longrightarrow> fv\<^sub>M\<^sub>L(comp_open t) = fv t"
 by(induct t pred:pure) (simp_all add:comp_open_def)
 
-lemma fv_ML_comp_pat: "pattern t \<Longrightarrow> fv\<^bsub>ML\<^esub>(comp_pat t) = fv t"
+lemma fv_ML_comp_pat: "pattern t \<Longrightarrow> fv\<^sub>M\<^sub>L(comp_pat t) = fv t"
 by(induct t pred:pattern)(simp_all add:comp_open_def)
 
 lemma fv_compR_aux:
-  "(nm,ts,t') : R \<Longrightarrow> x \<in> fv\<^bsub>ML\<^esub> (comp_open t')
-   \<Longrightarrow> \<exists>t\<in>set ts. x \<in> fv\<^bsub>ML\<^esub>(comp_pat t)"
+  "(nm,ts,t') : R \<Longrightarrow> x \<in> fv\<^sub>M\<^sub>L (comp_open t')
+   \<Longrightarrow> \<exists>t\<in>set ts. x \<in> fv\<^sub>M\<^sub>L(comp_pat t)"
 apply(frule pure_R)
 apply(simp add:fv_ML_comp_open)
 apply(frule (1) fv_R)
@@ -1156,7 +1156,7 @@ apply(simp add:fv_ML_comp_pat)
 done
 
 lemma fv_compR:
-  "(nm,vs,v) : compR \<Longrightarrow> x \<in> fv\<^bsub>ML\<^esub> v \<Longrightarrow> \<exists>u\<in>set vs. x \<in> fv\<^bsub>ML\<^esub> u"
+  "(nm,vs,v) : compR \<Longrightarrow> x \<in> fv\<^sub>M\<^sub>L v \<Longrightarrow> \<exists>u\<in>set vs. x \<in> fv\<^sub>M\<^sub>L u"
 by(fastforce simp add:compR_def image_def dest: fv_compR_aux)
 
 lemma lift_compile:
@@ -1170,11 +1170,11 @@ apply (clarsimp simp: lift_lift_ML_comm)
 done
 
 lemma subst_ML_compile:
-  "pure t \<Longrightarrow> subst\<^bsub>ML\<^esub> \<sigma>' (compile t \<sigma>) = compile t (subst\<^bsub>ML\<^esub> \<sigma>' o \<sigma>)"
+  "pure t \<Longrightarrow> subst\<^sub>M\<^sub>L \<sigma>' (compile t \<sigma>) = compile t (subst\<^sub>M\<^sub>L \<sigma>' o \<sigma>)"
 apply(induct arbitrary: \<sigma> \<sigma>' pred:pure)
 apply simp_all
-apply(erule_tac x="V\<^bsub>ML\<^esub> 0 ## \<sigma>'" in meta_allE)
-apply(erule_tac x= "V\<^bsub>ML\<^esub> 0 ## (lift\<^bsub>ML\<^esub> 0 \<circ> \<sigma>)" in meta_allE)
+apply(erule_tac x="V\<^sub>M\<^sub>L 0 ## \<sigma>'" in meta_allE)
+apply(erule_tac x= "V\<^sub>M\<^sub>L 0 ## (lift\<^sub>M\<^sub>L 0 \<circ> \<sigma>)" in meta_allE)
 apply(rule_tac f = "compile t" in arg_cong)
 apply(rule ext)
 apply (auto simp add:subst_ML_ext lift_ML_subst_ML)
@@ -1186,16 +1186,16 @@ apply(induct arbitrary: \<sigma> pred:pure)
 apply simp_all
 apply(subst lift_compile) apply simp
 apply(subst subst_ML_compile) apply simp
-apply(subgoal_tac "(subst\<^bsub>ML\<^esub> (\<lambda>n. if n = 0 then V\<^sub>U 0 [] else V\<^bsub>ML\<^esub> (n - 1)) \<circ>
-               (lift 0 \<circ> V\<^bsub>ML\<^esub> 0 ## \<sigma>)) = (\<lambda>a. V\<^sub>U a [])")
+apply(subgoal_tac "(subst\<^sub>M\<^sub>L (\<lambda>n. if n = 0 then V\<^sub>U 0 [] else V\<^sub>M\<^sub>L (n - 1)) \<circ>
+               (lift 0 \<circ> V\<^sub>M\<^sub>L 0 ## \<sigma>)) = (\<lambda>a. V\<^sub>U a [])")
 apply(simp)
 apply(rule ext)
 apply(simp)
 done
 
 lemma kernel_subst_ML_pat:
-  "pure t \<Longrightarrow> pattern t \<Longrightarrow> \<forall>i. closed\<^bsub>ML\<^esub> 0 (\<sigma> i) \<Longrightarrow>
-   (subst\<^bsub>ML\<^esub> \<sigma> (comp_pat t))! = subst (kernel \<circ> \<sigma>) t"
+  "pure t \<Longrightarrow> pattern t \<Longrightarrow> \<forall>i. closed\<^sub>M\<^sub>L 0 (\<sigma> i) \<Longrightarrow>
+   (subst\<^sub>M\<^sub>L \<sigma> (comp_pat t))! = subst (kernel \<circ> \<sigma>) t"
 apply(induct arbitrary: \<sigma> pred:pure)
 apply simp_all
 apply(frule pattern_At_decomp)
@@ -1206,13 +1206,13 @@ apply(simp add: rev_map)
 done
 
 lemma kernel_subst_ML:
-  "pure t \<Longrightarrow> \<forall>i. closed\<^bsub>ML\<^esub> 0 (\<sigma> i) \<Longrightarrow>
-   (subst\<^bsub>ML\<^esub> \<sigma> (comp_open t))! = subst (kernel \<circ> \<sigma>) t"
+  "pure t \<Longrightarrow> \<forall>i. closed\<^sub>M\<^sub>L 0 (\<sigma> i) \<Longrightarrow>
+   (subst\<^sub>M\<^sub>L \<sigma> (comp_open t))! = subst (kernel \<circ> \<sigma>) t"
 proof(induct arbitrary: \<sigma> pred:pure)
   case (Lam t)
-  have "lift 0 o V\<^bsub>ML\<^esub> = V\<^bsub>ML\<^esub>" by (simp add:fun_eq_iff)
-  hence "(subst\<^bsub>ML\<^esub> \<sigma> (comp_open (\<Lambda> t)))! =
-    \<Lambda> (subst\<^bsub>ML\<^esub> (lift 0 \<circ> V\<^bsub>ML\<^esub> 0 ## \<sigma>) (comp_open t)[V\<^sub>U 0 []/0]!)"
+  have "lift 0 o V\<^sub>M\<^sub>L = V\<^sub>M\<^sub>L" by (simp add:fun_eq_iff)
+  hence "(subst\<^sub>M\<^sub>L \<sigma> (comp_open (\<Lambda> t)))! =
+    \<Lambda> (subst\<^sub>M\<^sub>L (lift 0 \<circ> V\<^sub>M\<^sub>L 0 ## \<sigma>) (comp_open t)[V\<^sub>U 0 []/0]!)"
     using Lam by(simp add: lift_subst_ML comp_open_def lift_compile)
   also have "\<dots> = \<Lambda> (subst (V 0 ## (kernel \<circ> \<sigma>)) t)" using Lam
     by(simp add: subst_ML_comp subst_ext kernel_lift_tm)
@@ -1221,13 +1221,13 @@ proof(induct arbitrary: \<sigma> pred:pure)
 qed (simp_all add:comp_open_def)
 
 lemma kernel_subst_ML_pat_map:
-  "\<forall>t \<in> set ts. pure t \<Longrightarrow> patterns ts \<Longrightarrow> \<forall>i. closed\<^bsub>ML\<^esub> 0 (\<sigma> i) \<Longrightarrow>
-   map kernel (map (subst\<^bsub>ML\<^esub> \<sigma>) (map comp_pat ts)) =
+  "\<forall>t \<in> set ts. pure t \<Longrightarrow> patterns ts \<Longrightarrow> \<forall>i. closed\<^sub>M\<^sub>L 0 (\<sigma> i) \<Longrightarrow>
+   map kernel (map (subst\<^sub>M\<^sub>L \<sigma>) (map comp_pat ts)) =
    map (subst (kernel \<circ> \<sigma>)) ts"
 by(simp add:list_eq_iff_nth_eq kernel_subst_ML_pat)
 
-lemma compR_Red_tm: "(nm, vs, v) : compR \<Longrightarrow> \<forall> i. closed\<^bsub>ML\<^esub> 0 (\<sigma> i)
-  \<Longrightarrow> C nm \<bullet>\<bullet> (map (subst\<^bsub>ML\<^esub> \<sigma>) (rev vs))! \<rightarrow>* (subst\<^bsub>ML\<^esub> \<sigma> v)!"
+lemma compR_Red_tm: "(nm, vs, v) : compR \<Longrightarrow> \<forall> i. closed\<^sub>M\<^sub>L 0 (\<sigma> i)
+  \<Longrightarrow> C nm \<bullet>\<bullet> (map (subst\<^sub>M\<^sub>L \<sigma>) (rev vs))! \<rightarrow>* (subst\<^sub>M\<^sub>L \<sigma> v)!"
 apply(auto simp add:compR_def rev_map simp del: map_map)
 apply(frule pure_R)
 apply(subst kernel_subst_ML) apply fast+
@@ -1249,13 +1249,13 @@ by simp
 
 text{* Soundness of reduction: *}
 theorem fixes v :: ml shows Red_ml_sound:
-  "v \<Rightarrow> v' \<Longrightarrow> closed\<^bsub>ML\<^esub> 0 v \<Longrightarrow> v! \<rightarrow>* v'! \<and> closed\<^bsub>ML\<^esub> 0 v'" and
-  "vs \<Rightarrow> vs' \<Longrightarrow> \<forall>v\<in>set vs. closed\<^bsub>ML\<^esub> 0 v \<Longrightarrow>
-   vs! \<rightarrow>* vs'! \<and> (\<forall>v'\<in>set vs'. closed\<^bsub>ML\<^esub> 0 v')"
+  "v \<Rightarrow> v' \<Longrightarrow> closed\<^sub>M\<^sub>L 0 v \<Longrightarrow> v! \<rightarrow>* v'! \<and> closed\<^sub>M\<^sub>L 0 v'" and
+  "vs \<Rightarrow> vs' \<Longrightarrow> \<forall>v\<in>set vs. closed\<^sub>M\<^sub>L 0 v \<Longrightarrow>
+   vs! \<rightarrow>* vs'! \<and> (\<forall>v'\<in>set vs'. closed\<^sub>M\<^sub>L 0 v')"
 proof(induct rule:Red_ml_Red_ml_list.inducts)
   fix u v
-  let ?v = "A\<^bsub>ML\<^esub> (Lam\<^bsub>ML\<^esub> u) [v]"
-  assume cl: "closed\<^bsub>ML\<^esub> 0 (A\<^bsub>ML\<^esub> (Lam\<^bsub>ML\<^esub> u) [v])"
+  let ?v = "A\<^sub>M\<^sub>L (Lam\<^sub>M\<^sub>L u) [v]"
+  assume cl: "closed\<^sub>M\<^sub>L 0 (A\<^sub>M\<^sub>L (Lam\<^sub>M\<^sub>L u) [v])"
   let ?u' = "(lift_ml 0 u)[V\<^sub>U 0 []/0]"
   have "?v! = (\<Lambda>((?u')!)) \<bullet> (v !)" by simp
   also have "\<dots> \<rightarrow> (?u' !)[v!/0]" (is "_ \<rightarrow> ?R") by(rule Red_tm.intros)
@@ -1263,37 +1263,37 @@ proof(induct rule:Red_ml_Red_ml_list.inducts)
     apply(cut_tac u = "u" and v = "v" in kernel_subst1)
     apply(simp_all)
     done
-  finally have "kernel(A\<^bsub>ML\<^esub> (Lam\<^bsub>ML\<^esub> u) [v]) \<rightarrow>* kernel(u[v/0])" (is ?A)
+  finally have "kernel(A\<^sub>M\<^sub>L (Lam\<^sub>M\<^sub>L u) [v]) \<rightarrow>* kernel(u[v/0])" (is ?A)
     by(rule r_into_rtrancl)
-  moreover have "closed\<^bsub>ML\<^esub> 0 (u[v/0])" (is "?C")
+  moreover have "closed\<^sub>M\<^sub>L 0 (u[v/0])" (is "?C")
   proof -
-    let ?\<sigma> = "\<lambda>n. if n = 0 then v else V\<^bsub>ML\<^esub> (n - 1)"
+    let ?\<sigma> = "\<lambda>n. if n = 0 then v else V\<^sub>M\<^sub>L (n - 1)"
     let ?\<sigma>' = "\<lambda>n. v"
-    have clu: "closed\<^bsub>ML\<^esub> (Suc 0) u" and clv: "closed\<^bsub>ML\<^esub> 0 v" using cl by simp+
-    have "closed\<^bsub>ML\<^esub> 0 (subst\<^bsub>ML\<^esub> ?\<sigma>' u)"
+    have clu: "closed\<^sub>M\<^sub>L (Suc 0) u" and clv: "closed\<^sub>M\<^sub>L 0 v" using cl by simp+
+    have "closed\<^sub>M\<^sub>L 0 (subst\<^sub>M\<^sub>L ?\<sigma>' u)"
       by (metis closed_ML_subst_ML clv)
-    hence "closed\<^bsub>ML\<^esub> 0 (subst\<^bsub>ML\<^esub> ?\<sigma> u)"
+    hence "closed\<^sub>M\<^sub>L 0 (subst\<^sub>M\<^sub>L ?\<sigma> u)"
       using subst_ML_coincidence[OF clu, of ?\<sigma> ?\<sigma>'] by auto
     thus ?thesis by simp
   qed
   ultimately show "?A \<and> ?C" ..
 next
   fix \<sigma> :: "nat \<Rightarrow> ml" and nm vs v
-  assume \<sigma>: "\<forall>i. closed\<^bsub>ML\<^esub> 0 (\<sigma> i)"  and compR: "(nm, vs, v) \<in> compR"
-  have "map (subst V) (map (subst\<^bsub>ML\<^esub> \<sigma>) (rev vs)!) = map (subst\<^bsub>ML\<^esub> \<sigma>) (rev vs)!"
+  assume \<sigma>: "\<forall>i. closed\<^sub>M\<^sub>L 0 (\<sigma> i)"  and compR: "(nm, vs, v) \<in> compR"
+  have "map (subst V) (map (subst\<^sub>M\<^sub>L \<sigma>) (rev vs)!) = map (subst\<^sub>M\<^sub>L \<sigma>) (rev vs)!"
     by(simp add:list_eq_iff_nth_eq subst_V_kernel closed_ML_subst_ML[OF \<sigma>])
   with compR_Red_tm[OF compR \<sigma>]
-  have "(C nm) \<bullet>\<bullet> ((map (subst\<^bsub>ML\<^esub> \<sigma>) (rev vs)) !) \<rightarrow>* (subst\<^bsub>ML\<^esub> \<sigma> v)!"
+  have "(C nm) \<bullet>\<bullet> ((map (subst\<^sub>M\<^sub>L \<sigma>) (rev vs)) !) \<rightarrow>* (subst\<^sub>M\<^sub>L \<sigma> v)!"
     by(simp add:subst_V_kernel closed_ML_subst_ML[OF \<sigma>])
-  hence "A\<^bsub>ML\<^esub> (C\<^bsub>ML\<^esub> nm) (map (subst\<^bsub>ML\<^esub> \<sigma>) vs)! \<rightarrow>* subst\<^bsub>ML\<^esub> \<sigma> v!" (is ?A)
+  hence "A\<^sub>M\<^sub>L (C\<^sub>M\<^sub>L nm) (map (subst\<^sub>M\<^sub>L \<sigma>) vs)! \<rightarrow>* subst\<^sub>M\<^sub>L \<sigma> v!" (is ?A)
     by(simp add:rev_map)
   moreover
-  have "closed\<^bsub>ML\<^esub> 0 (subst\<^bsub>ML\<^esub> \<sigma> v)" (is ?C) by(metis closed_ML_subst_ML \<sigma>)
+  have "closed\<^sub>M\<^sub>L 0 (subst\<^sub>M\<^sub>L \<sigma> v)" (is ?C) by(metis closed_ML_subst_ML \<sigma>)
   ultimately show "?A \<and> ?C" ..
 qed (auto simp:Reds_tm_list_foldl_At Red_tm_rev rev_map[symmetric])
 
 theorem Red_term_sound:
-  "t \<Rightarrow> t' \<Longrightarrow> closed\<^bsub>ML\<^esub> 0 t \<Longrightarrow> kernelt t \<rightarrow>* kernelt t'  \<and> closed\<^bsub>ML\<^esub> 0 t'"
+  "t \<Rightarrow> t' \<Longrightarrow> closed\<^sub>M\<^sub>L 0 t \<Longrightarrow> kernelt t \<rightarrow>* kernelt t'  \<and> closed\<^sub>M\<^sub>L 0 t'"
 proof(induct rule:Red_term.inducts)
   case term_C thus ?case
     by (auto simp:closed_tm_ML_foldl_At)
@@ -1312,7 +1312,7 @@ next
     using term_Clo
     by(simp del:lift_foldl_At add: r_into_rtrancl Red_tm.intros(2))
   moreover
-  have "closed\<^bsub>ML\<^esub> 0 (\<Lambda> (term (apply (lift 0 (Clo vf vs n)) (V\<^sub>U 0 []))))"
+  have "closed\<^sub>M\<^sub>L 0 (\<Lambda> (term (apply (lift 0 (Clo vf vs n)) (V\<^sub>U 0 []))))"
     using term_Clo by simp
   ultimately show ?case ..
 next
@@ -1320,17 +1320,17 @@ next
 qed auto
 
 corollary kernel_inv:
- "(t :: tm) \<Rightarrow>* t' \<Longrightarrow> closed\<^bsub>ML\<^esub> 0 t \<Longrightarrow> t! \<rightarrow>* t'! \<and> closed\<^bsub>ML\<^esub> 0 t' "
+ "(t :: tm) \<Rightarrow>* t' \<Longrightarrow> closed\<^sub>M\<^sub>L 0 t \<Longrightarrow> t! \<rightarrow>* t'! \<and> closed\<^sub>M\<^sub>L 0 t' "
 apply(induct rule: rtrancl.induct)
 apply (metis rtrancl_eq_or_trancl)
 apply (metis Red_term_sound rtrancl_trans)
 done
 
 lemma  closed_ML_compile:
-  "pure t \<Longrightarrow> \<forall>i. closed\<^bsub>ML\<^esub> n (\<sigma> i) \<Longrightarrow> closed\<^bsub>ML\<^esub> n (compile t \<sigma>)"
+  "pure t \<Longrightarrow> \<forall>i. closed\<^sub>M\<^sub>L n (\<sigma> i) \<Longrightarrow> closed\<^sub>M\<^sub>L n (compile t \<sigma>)"
 proof(induct arbitrary:n \<sigma> pred:pure)
   case (Lam t)
-  have 1: "\<forall>i. closed\<^bsub>ML\<^esub> (Suc n) ((V\<^bsub>ML\<^esub> 0 ## \<sigma>) i)" using Lam(3-)
+  have 1: "\<forall>i. closed\<^sub>M\<^sub>L (Suc n) ((V\<^sub>M\<^sub>L 0 ## \<sigma>) i)" using Lam(3-)
     by (auto simp: closed_ML_Suc)
   show ?case using Lam(2)[OF 1] by (simp del:apply_cons_ML)
 qed simp_all
@@ -1338,7 +1338,7 @@ qed simp_all
 theorem nbe_correct: fixes t :: tm
 assumes "pure t" and "term (comp_fixed t) \<Rightarrow>* t'" and "pure t'" shows "t \<rightarrow>* t'"
 proof -
-  have ML_cl: "closed\<^bsub>ML\<^esub> 0 (term (comp_fixed t))"
+  have ML_cl: "closed\<^sub>M\<^sub>L 0 (term (comp_fixed t))"
     by (simp add: closed_ML_compile[OF `pure t`])
   have "(term (comp_fixed t))! = t"
     using kernel_compile[OF `pure t`] by simp
@@ -1358,16 +1358,16 @@ inductive normal :: "tm \<Rightarrow> bool" where
  \<forall>\<sigma>. \<forall>(nm',ls,r)\<in>R. \<not>(nm = nm' \<and> take (size ls) ts = map (subst \<sigma>) ls)
  \<Longrightarrow> normal(C nm \<bullet>\<bullet> ts)"
 
-fun C_normal_ML :: "ml \<Rightarrow> bool" ("C'_normal\<^bsub>ML\<^esub>") where
-"C_normal\<^bsub>ML\<^esub>(C\<^sub>U nm vs) =
-  ((\<forall>v\<in>set vs. C_normal\<^bsub>ML\<^esub> v) \<and> no_match_compR nm vs)" |
-"C_normal\<^bsub>ML\<^esub> (C\<^bsub>ML\<^esub> _) = True" |
-"C_normal\<^bsub>ML\<^esub> (V\<^bsub>ML\<^esub> _) = True" |
-"C_normal\<^bsub>ML\<^esub> (A\<^bsub>ML\<^esub> v vs) = (C_normal\<^bsub>ML\<^esub> v \<and> (\<forall>v \<in> set vs. C_normal\<^bsub>ML\<^esub> v))" |
-"C_normal\<^bsub>ML\<^esub> (Lam\<^bsub>ML\<^esub> v) = C_normal\<^bsub>ML\<^esub> v" |
-"C_normal\<^bsub>ML\<^esub> (V\<^sub>U x vs) = (\<forall>v \<in> set vs. C_normal\<^bsub>ML\<^esub> v)" |
-"C_normal\<^bsub>ML\<^esub> (Clo v vs _) = (C_normal\<^bsub>ML\<^esub> v \<and> (\<forall>v \<in> set vs. C_normal\<^bsub>ML\<^esub> v))" |
-"C_normal\<^bsub>ML\<^esub> (apply u v) = (C_normal\<^bsub>ML\<^esub> u \<and> C_normal\<^bsub>ML\<^esub> v)"
+fun C_normal_ML :: "ml \<Rightarrow> bool" ("C'_normal\<^sub>M\<^sub>L") where
+"C_normal\<^sub>M\<^sub>L(C\<^sub>U nm vs) =
+  ((\<forall>v\<in>set vs. C_normal\<^sub>M\<^sub>L v) \<and> no_match_compR nm vs)" |
+"C_normal\<^sub>M\<^sub>L (C\<^sub>M\<^sub>L _) = True" |
+"C_normal\<^sub>M\<^sub>L (V\<^sub>M\<^sub>L _) = True" |
+"C_normal\<^sub>M\<^sub>L (A\<^sub>M\<^sub>L v vs) = (C_normal\<^sub>M\<^sub>L v \<and> (\<forall>v \<in> set vs. C_normal\<^sub>M\<^sub>L v))" |
+"C_normal\<^sub>M\<^sub>L (Lam\<^sub>M\<^sub>L v) = C_normal\<^sub>M\<^sub>L v" |
+"C_normal\<^sub>M\<^sub>L (V\<^sub>U x vs) = (\<forall>v \<in> set vs. C_normal\<^sub>M\<^sub>L v)" |
+"C_normal\<^sub>M\<^sub>L (Clo v vs _) = (C_normal\<^sub>M\<^sub>L v \<and> (\<forall>v \<in> set vs. C_normal\<^sub>M\<^sub>L v))" |
+"C_normal\<^sub>M\<^sub>L (apply u v) = (C_normal\<^sub>M\<^sub>L u \<and> C_normal\<^sub>M\<^sub>L v)"
 
 fun size_tm :: "tm \<Rightarrow> nat" where
 "size_tm (C _) = 1" |
@@ -1421,16 +1421,16 @@ apply(subst no_match.simps)
 apply fastforce
 done
 
-fun dterm_ML :: "ml \<Rightarrow> tm" ("dterm\<^bsub>ML\<^esub>") where
-"dterm\<^bsub>ML\<^esub> (C\<^sub>U nm vs) = C nm \<bullet>\<bullet> map dterm\<^bsub>ML\<^esub> (rev vs)" |
-"dterm\<^bsub>ML\<^esub> _ = V 0"
+fun dterm_ML :: "ml \<Rightarrow> tm" ("dterm\<^sub>M\<^sub>L") where
+"dterm\<^sub>M\<^sub>L (C\<^sub>U nm vs) = C nm \<bullet>\<bullet> map dterm\<^sub>M\<^sub>L (rev vs)" |
+"dterm\<^sub>M\<^sub>L _ = V 0"
 
 fun dterm :: "tm \<Rightarrow> tm" where
 "dterm (V n) = V n" |
 "dterm (C nm) = C nm" |
 "dterm (s \<bullet> t) = dterm s \<bullet> dterm t" |
 "dterm (\<Lambda> t) = \<Lambda> (dterm t)" |
-"dterm (term v) = dterm\<^bsub>ML\<^esub> v"
+"dterm (term v) = dterm\<^sub>M\<^sub>L v"
 
 lemma dterm_pure[simp]: "pure t \<Longrightarrow> dterm t = t"
 by (induct pred:pure) auto
@@ -1438,15 +1438,15 @@ by (induct pred:pure) auto
 lemma map_dterm_pure[simp]: "\<forall>t\<in>set ts. pure t \<Longrightarrow> map dterm ts = ts"
 by (induct ts) auto
 
-lemma map_dterm_term[simp]: "map dterm (map term vs) = map dterm\<^bsub>ML\<^esub> vs"
+lemma map_dterm_term[simp]: "map dterm (map term vs) = map dterm\<^sub>M\<^sub>L vs"
 by (induct vs) auto
 
 lemma dterm_foldl_At[simp]: "dterm(t \<bullet>\<bullet> ts) = dterm t \<bullet>\<bullet> map dterm ts"
 by(induct ts arbitrary: t) auto
 
 lemma no_match_coincide:
-  "no_match\<^bsub>ML\<^esub> ps vs \<Longrightarrow>
-  no_match (map dterm\<^bsub>ML\<^esub> (rev ps)) (map dterm\<^bsub>ML\<^esub> (rev vs))"
+  "no_match\<^sub>M\<^sub>L ps vs \<Longrightarrow>
+  no_match (map dterm\<^sub>M\<^sub>L (rev ps)) (map dterm\<^sub>M\<^sub>L (rev vs))"
 apply(induct ps vs rule:no_match_ML.induct)
 apply(rotate_tac 1)
 apply(subst (asm) no_match_ML.simps)
@@ -1472,17 +1472,17 @@ apply (simp (no_asm))
 apply (metis min_less_iff_conj)
 apply(rule_tac x=nm' in exI)
 apply(rule_tac x=nm' in exI)
-apply(rule_tac x="map dterm\<^bsub>ML\<^esub> (rev vs)" in exI)
-apply(rule_tac x="map dterm\<^bsub>ML\<^esub> (rev vs')" in exI)
+apply(rule_tac x="map dterm\<^sub>M\<^sub>L (rev vs)" in exI)
+apply(rule_tac x="map dterm\<^sub>M\<^sub>L (rev vs')" in exI)
 apply(simp)
 done
 
 lemma dterm_ML_comp_patD:
-  "pattern t \<Longrightarrow> dterm\<^bsub>ML\<^esub> (comp_pat t) = C nm \<bullet>\<bullet> rs \<Longrightarrow> \<exists>ts. t = C nm \<bullet>\<bullet> ts"
+  "pattern t \<Longrightarrow> dterm\<^sub>M\<^sub>L (comp_pat t) = C nm \<bullet>\<bullet> rs \<Longrightarrow> \<exists>ts. t = C nm \<bullet>\<bullet> ts"
 by(induct pred:pattern) simp_all
 
 lemma no_match_R_coincide_aux[rule_format]: "patterns ts \<Longrightarrow>
-  no_match (map (dterm\<^bsub>ML\<^esub> \<circ> comp_pat) ts) rs \<longrightarrow> no_match ts rs"
+  no_match (map (dterm\<^sub>M\<^sub>L \<circ> comp_pat) ts) rs \<longrightarrow> no_match ts rs"
 apply(induct ts rs rule:no_match.induct)
 apply(subst (1 2) no_match.simps)
 apply clarsimp
@@ -1501,7 +1501,7 @@ apply (metis in_set_conv_nth pattern_At_vecD)
 done
 
 lemma no_match_R_coincide:
-  "no_match_compR nm (rev vs) \<Longrightarrow> no_match_R nm (map dterm\<^bsub>ML\<^esub> vs)"
+  "no_match_compR nm (rev vs) \<Longrightarrow> no_match_R nm (map dterm\<^sub>M\<^sub>L vs)"
 apply auto
 apply(drule_tac x="(nm, map comp_pat (rev aa), comp_open b)" in bspec)
  unfolding compR_def
@@ -1511,7 +1511,7 @@ apply (simp)
 apply(drule no_match_coincide)
 apply(frule pure_R)
 apply(drule pattern_R)
-apply(clarsimp simp add: rev_map no_match.simps[of _ "map dterm\<^bsub>ML\<^esub> vs"])
+apply(clarsimp simp add: rev_map no_match.simps[of _ "map dterm\<^sub>M\<^sub>L vs"])
 apply(rule_tac x=i in exI)
 apply simp
 apply(cut_tac t = "aa!i" in dterm_ML_comp_patD, simp, assumption)
@@ -1526,13 +1526,13 @@ done
 inductive C_normal :: "tm \<Rightarrow> bool" where
 "\<forall>t\<in>set ts. C_normal t \<Longrightarrow> C_normal(V x \<bullet>\<bullet> ts)" |
 "C_normal t \<Longrightarrow> C_normal(\<Lambda> t)" |
-"C_normal\<^bsub>ML\<^esub> v \<Longrightarrow> C_normal(term v)" |
+"C_normal\<^sub>M\<^sub>L v \<Longrightarrow> C_normal(term v)" |
 "\<forall>t\<in>set ts. C_normal t \<Longrightarrow> no_match_R nm (map dterm ts)
  \<Longrightarrow> C_normal(C nm \<bullet>\<bullet> ts)"
 
 declare C_normal.intros[simp]
 
-lemma C_normal_term[simp]: "C_normal(term v) = C_normal\<^bsub>ML\<^esub> v"
+lemma C_normal_term[simp]: "C_normal(term v) = C_normal\<^sub>M\<^sub>L v"
 apply (auto)
 apply(erule C_normal.cases)
 apply auto
@@ -1548,7 +1548,7 @@ lemma [simp]: "C_normal(V x)"
 using C_normal.intros(1)[of "[]" x]
 by simp
 
-lemma [simp]: "dterm (dterm\<^bsub>ML\<^esub> v) = dterm\<^bsub>ML\<^esub> v"
+lemma [simp]: "dterm (dterm\<^sub>M\<^sub>L v) = dterm\<^sub>M\<^sub>L v"
 apply(induct v rule:dterm_ML.induct)
 apply simp_all
 done
@@ -1565,7 +1565,7 @@ apply (auto split:nat.splits)
 done
 
 lemma Red_ml_list_pres_no_match:
-  "no_match\<^bsub>ML\<^esub> ps vs \<Longrightarrow> vs \<Rightarrow> vs' \<Longrightarrow> no_match\<^bsub>ML\<^esub> ps vs'"
+  "no_match\<^sub>M\<^sub>L ps vs \<Longrightarrow> vs \<Rightarrow> vs' \<Longrightarrow> no_match\<^sub>M\<^sub>L ps vs'"
 proof(induct ps vs arbitrary: vs' rule:no_match_ML.induct)
   case (1 vs os)
   show ?case using 1(2-3)
@@ -1594,8 +1594,8 @@ done
 qed
 
 lemma no_match_ML_subst_ML[rule_format]:
-  "\<forall>v\<in>set vs. \<forall>x\<in>fv\<^bsub>ML\<^esub> v. C_normal\<^bsub>ML\<^esub> (\<sigma> x) \<Longrightarrow>
-   no_match\<^bsub>ML\<^esub> ps vs \<longrightarrow> no_match\<^bsub>ML\<^esub> ps (map (subst\<^bsub>ML\<^esub> \<sigma>) vs)"
+  "\<forall>v\<in>set vs. \<forall>x\<in>fv\<^sub>M\<^sub>L v. C_normal\<^sub>M\<^sub>L (\<sigma> x) \<Longrightarrow>
+   no_match\<^sub>M\<^sub>L ps vs \<longrightarrow> no_match\<^sub>M\<^sub>L ps (map (subst\<^sub>M\<^sub>L \<sigma>) vs)"
 apply(induct ps vs rule:no_match_ML.induct)
 apply simp
 apply(subst (1 2) no_match_ML.simps)
@@ -1603,7 +1603,7 @@ apply clarsimp
 apply(rule_tac x=i in exI)
 apply simp
 apply(rule_tac x=nm' in exI)
-apply(rule_tac x="map (subst\<^bsub>ML\<^esub> \<sigma>) vs'" in exI)
+apply(rule_tac x="map (subst\<^sub>M\<^sub>L \<sigma>) vs'" in exI)
 apply (auto simp:rev_nth)
 apply(erule_tac x = i in meta_allE)
 apply(erule_tac x = nm' in meta_allE)
@@ -1615,11 +1615,11 @@ apply (metis UN_I fv_ML.simps(5) in_set_conv_nth length_rev rev_nth set_rev)
 done
 
 lemma lift_is_CUD:
-  "lift\<^bsub>ML\<^esub> k v = C\<^sub>U nm vs' \<Longrightarrow> \<exists>vs. v = C\<^sub>U nm vs \<and> vs' = map (lift\<^bsub>ML\<^esub> k) vs"
+  "lift\<^sub>M\<^sub>L k v = C\<^sub>U nm vs' \<Longrightarrow> \<exists>vs. v = C\<^sub>U nm vs \<and> vs' = map (lift\<^sub>M\<^sub>L k) vs"
 by(cases v) auto
 
 lemma no_match_ML_lift_ML:
-  "no_match\<^bsub>ML\<^esub> ps (map (lift\<^bsub>ML\<^esub> k) vs) = no_match\<^bsub>ML\<^esub> ps vs"
+  "no_match\<^sub>M\<^sub>L ps (map (lift\<^sub>M\<^sub>L k) vs) = no_match\<^sub>M\<^sub>L ps vs"
 apply(induct ps vs rule:no_match_ML.induct)
 apply simp
 apply(subst (1 2) no_match_ML.simps)
@@ -1633,11 +1633,11 @@ apply clarsimp
 apply(rule_tac x=i in exI)
 apply simp
 apply(rule_tac x=nm' in exI)
-apply(rule_tac x="map (lift\<^bsub>ML\<^esub> k) vs'" in exI)
+apply(rule_tac x="map (lift\<^sub>M\<^sub>L k) vs'" in exI)
 apply (fastforce simp:rev_nth)
 done
 
-lemma C_normal_ML_lift_ML: "C_normal\<^bsub>ML\<^esub>(lift\<^bsub>ML\<^esub> k v) = C_normal\<^bsub>ML\<^esub> v"
+lemma C_normal_ML_lift_ML: "C_normal\<^sub>M\<^sub>L(lift\<^sub>M\<^sub>L k v) = C_normal\<^sub>M\<^sub>L v"
 by(induct v arbitrary: k rule:C_normal_ML.induct)(auto simp:no_match_ML_lift_ML)
 
 lemma no_match_compR_Cons:
@@ -1652,23 +1652,23 @@ apply(rule_tac x=i in exI)
 apply (simp add:nth_append)
 done
 
-lemma C_normal_ML_comp_open: "pure t \<Longrightarrow> C_normal\<^bsub>ML\<^esub>(comp_open t)"
+lemma C_normal_ML_comp_open: "pure t \<Longrightarrow> C_normal\<^sub>M\<^sub>L(comp_open t)"
 by (induct pred:pure) (auto simp:comp_open_def)
 
-lemma C_normal_compR_rhs: "(nm, vs, v) \<in> compR \<Longrightarrow> C_normal\<^bsub>ML\<^esub> v"
+lemma C_normal_compR_rhs: "(nm, vs, v) \<in> compR \<Longrightarrow> C_normal\<^sub>M\<^sub>L v"
 by(auto simp: compR_def image_def Bex_def pure_R C_normal_ML_comp_open)
 
 
 lemma C_normal_ML_subst_ML:
-  "C_normal\<^bsub>ML\<^esub> (subst\<^bsub>ML\<^esub> \<sigma> v) \<Longrightarrow> (\<forall>x\<in>fv\<^bsub>ML\<^esub> v. C_normal\<^bsub>ML\<^esub> (\<sigma> x))"
+  "C_normal\<^sub>M\<^sub>L (subst\<^sub>M\<^sub>L \<sigma> v) \<Longrightarrow> (\<forall>x\<in>fv\<^sub>M\<^sub>L v. C_normal\<^sub>M\<^sub>L (\<sigma> x))"
 proof(induct \<sigma> v rule:subst_ML.induct)
   case 4 thus ?case
     by(simp del:apply_cons_ML)(force simp add: C_normal_ML_lift_ML)
       (* weird - force suffices in apply style *)
 qed auto
 
-lemma C_normal_ML_subst_ML_iff: "C_normal\<^bsub>ML\<^esub> v \<Longrightarrow>
-  C_normal\<^bsub>ML\<^esub> (subst\<^bsub>ML\<^esub> \<sigma> v) \<longleftrightarrow> (\<forall>x\<in>fv\<^bsub>ML\<^esub> v. C_normal\<^bsub>ML\<^esub> (\<sigma> x))"
+lemma C_normal_ML_subst_ML_iff: "C_normal\<^sub>M\<^sub>L v \<Longrightarrow>
+  C_normal\<^sub>M\<^sub>L (subst\<^sub>M\<^sub>L \<sigma> v) \<longleftrightarrow> (\<forall>x\<in>fv\<^sub>M\<^sub>L v. C_normal\<^sub>M\<^sub>L (\<sigma> x))"
 proof(induct \<sigma> v rule:subst_ML.induct)
   case 4 thus ?case
     by(simp del:apply_cons_ML)(force simp add: C_normal_ML_lift_ML)
@@ -1677,8 +1677,8 @@ next
   case 5 thus ?case by simp (blast intro: no_match_ML_subst_ML)
 qed auto
 
-lemma C_normal_ML_inv: "v \<Rightarrow> v' \<Longrightarrow> C_normal\<^bsub>ML\<^esub> v \<Longrightarrow> C_normal\<^bsub>ML\<^esub> v'" and
-      "vs \<Rightarrow> vs' \<Longrightarrow> \<forall>v\<in>set vs. C_normal\<^bsub>ML\<^esub> v \<Longrightarrow> \<forall>v'\<in>set vs'. C_normal\<^bsub>ML\<^esub> v'"
+lemma C_normal_ML_inv: "v \<Rightarrow> v' \<Longrightarrow> C_normal\<^sub>M\<^sub>L v \<Longrightarrow> C_normal\<^sub>M\<^sub>L v'" and
+      "vs \<Rightarrow> vs' \<Longrightarrow> \<forall>v\<in>set vs. C_normal\<^sub>M\<^sub>L v \<Longrightarrow> \<forall>v'\<in>set vs'. C_normal\<^sub>M\<^sub>L v'"
 apply(induct rule:Red_ml_Red_ml_list.inducts)
 apply(simp_all add: C_normal_ML_subst_ML_iff)
   apply(metis C_normal_ML_subst_ML C_normal_compR_rhs
@@ -1767,7 +1767,7 @@ apply metis+
 done
 
 
-lemma [simp]: "C_normal(term v \<bullet>\<bullet> ts) \<longleftrightarrow> C_normal\<^bsub>ML\<^esub> v \<and> ts = []"
+lemma [simp]: "C_normal(term v \<bullet>\<bullet> ts) \<longleftrightarrow> C_normal\<^sub>M\<^sub>L v \<and> ts = []"
 by(fastforce elim: C_normal.cases)
 
 lemma [simp]: "C_normal(\<Lambda> t \<bullet>\<bullet> ts) \<longleftrightarrow> C_normal t \<and> ts = []"
@@ -1781,7 +1781,7 @@ lemma [simp]: "C_normal(V x \<bullet>\<bullet> ts) \<longleftrightarrow> (\<fora
 by(fastforce elim: C_normal.cases)
 
 lemma no_match_ML_lift:
-  "no_match\<^bsub>ML\<^esub> ps vs \<longrightarrow> no_match\<^bsub>ML\<^esub> ps (map (lift k) vs)"
+  "no_match\<^sub>M\<^sub>L ps vs \<longrightarrow> no_match\<^sub>M\<^sub>L ps (map (lift k) vs)"
 apply(induct ps vs rule:no_match_ML.induct)
 apply simp
 apply(subst (1 2) no_match_ML.simps)
@@ -1797,7 +1797,7 @@ lemma no_match_compR_lift:
   "no_match_compR nm vs \<Longrightarrow> no_match_compR nm (map (lift k) vs)"
 by (fastforce simp: no_match_ML_lift)
 
-lemma [simp]: "C_normal\<^bsub>ML\<^esub> v \<Longrightarrow> C_normal\<^bsub>ML\<^esub>(lift k v)"
+lemma [simp]: "C_normal\<^sub>M\<^sub>L v \<Longrightarrow> C_normal\<^sub>M\<^sub>L(lift k v)"
 apply(induct v arbitrary:k rule:lift_ml.induct)
 apply(simp_all add:no_match_compR_lift)
 done
@@ -1828,7 +1828,7 @@ proof(induct ps dts arbitrary: ts i t' rule:no_match.induct)
         proof(cases rule:Red_term_hnf_cases)
           case (5 v v' ts'')
           then obtain vs where [simp]:
-            "v = C\<^sub>U nm' vs" "rs' = map dterm\<^bsub>ML\<^esub> (rev vs) @ map dterm ts''"
+            "v = C\<^sub>U nm' vs" "rs' = map dterm\<^sub>M\<^sub>L (rev vs) @ map dterm ts''"
             using ob by(cases v) auto
           obtain vs' where [simp]: "v' = C\<^sub>U nm' vs'" "vs \<Rightarrow> vs'"
             using `v\<Rightarrow>v'` by(rule Red_ml.cases) auto
@@ -1861,7 +1861,7 @@ proof(induct ps dts arbitrary: ts i t' rule:no_match.induct)
           qed
         next
           case (9 v k r' ts'')
-          then obtain vs where [simp]: "v = C\<^sub>U nm' vs" "rs' = map dterm\<^bsub>ML\<^esub> (rev vs) @ map dterm ts''"
+          then obtain vs where [simp]: "v = C\<^sub>U nm' vs" "rs' = map dterm\<^sub>M\<^sub>L (rev vs) @ map dterm ts''"
             using ob by(cases v) auto
           show ?thesis (is "\<exists>rs'. ?P rs' \<and> ?Q rs'")
           proof
@@ -1954,8 +1954,8 @@ apply(fast intro: converse_rtrancl_into_rtrancl dest: ctxt_term)
 done
 
 lemma C_Red_term_ML:
-  "v \<Rightarrow> v' \<Longrightarrow> C_normal\<^bsub>ML\<^esub> v \<Longrightarrow> dterm\<^bsub>ML\<^esub> v = C nm \<bullet>\<bullet> ts
-   \<Longrightarrow> dterm\<^bsub>ML\<^esub> v' = C nm \<bullet>\<bullet> map dterm (C\<^sub>U_args(term v')) \<and>
+  "v \<Rightarrow> v' \<Longrightarrow> C_normal\<^sub>M\<^sub>L v \<Longrightarrow> dterm\<^sub>M\<^sub>L v = C nm \<bullet>\<bullet> ts
+   \<Longrightarrow> dterm\<^sub>M\<^sub>L v' = C nm \<bullet>\<bullet> map dterm (C\<^sub>U_args(term v')) \<and>
       C\<^sub>U_args(term v) [\<Rightarrow>*] C\<^sub>U_args(term v') \<and>
       ts = map dterm (C\<^sub>U_args(term v))" and
   "(vs:: ml list) \<Rightarrow> vs' \<Longrightarrow> i < length vs \<Longrightarrow> vs ! i \<Rightarrow>* vs' ! i"
@@ -2215,11 +2215,11 @@ lemma pure_foldl_At[simp]: "pure(s \<bullet>\<bullet> ts) \<longleftrightarrow> 
 by(induct ts arbitrary: s) auto
 
 lemma nbe_C_normal_ML:
-  assumes "term v \<Rightarrow>* t'" "C_normal\<^bsub>ML\<^esub> v" "pure t'" shows "normal t'"
+  assumes "term v \<Rightarrow>* t'" "C_normal\<^sub>M\<^sub>L v" "pure t'" shows "normal t'"
 proof -
   { fix t t' i v
     assume "(t,t') : Red_term^^i"
-    hence "t = term v \<Longrightarrow> C_normal\<^bsub>ML\<^esub> v \<Longrightarrow> pure t' \<Longrightarrow> normal t'"
+    hence "t = term v \<Longrightarrow> C_normal\<^sub>M\<^sub>L v \<Longrightarrow> pure t' \<Longrightarrow> normal t'"
     proof(induct i arbitrary: t t' v rule:less_induct)
     case (less k)
     show ?case
@@ -2305,7 +2305,7 @@ proof -
           then have "is!j < k" using `k=Suc i` 2 by auto
           have red: "(term (rev vs ! j), ts ! j) \<in> Red_term ^^ is ! j" using `j < ?n` 2 by auto
           have pure: "pure (ts ! j)" using `pure t'` 0 2 by auto
-          have Cnm: "C_normal\<^bsub>ML\<^esub> (rev vs ! j)" using less term_V
+          have Cnm: "C_normal\<^sub>M\<^sub>L (rev vs ! j)" using less term_V
             by simp (metis 0 in_set_conv_nth length_rev set_rev)
           from less(1)[OF `is!j < k` refl Cnm pure red] show "normal(ts!j)" .
         qed
@@ -2319,15 +2319,15 @@ proof -
           by(metis Lam_Red_term_itE)
         have "i' < k" using `k = Suc i` by arith
         have "pure t''" using `pure t'` by simp
-        have "C_normal\<^bsub>ML\<^esub> ?u" using less term_Clo by(simp)
-        from less(1)[OF `i' < k` refl `C_normal\<^bsub>ML\<^esub> ?u` `pure t''` 1]
+        have "C_normal\<^sub>M\<^sub>L ?u" using less term_Clo by(simp)
+        from less(1)[OF `i' < k` refl `C_normal\<^sub>M\<^sub>L ?u` `pure t''` 1]
         show ?thesis by(simp add:normal.intros)
       next
         case (ctxt_term u')
         have "i' < k" using `k = Suc i` by arith
-        have "C_normal\<^bsub>ML\<^esub> u'" by (rule C_normal_ML_inv) (insert less ctxt_term, simp_all)
+        have "C_normal\<^sub>M\<^sub>L u'" by (rule C_normal_ML_inv) (insert less ctxt_term, simp_all)
         have "(term u', t') \<in> Red_term ^^ i'" using red ctxt_term by auto
-        from less(1)[OF `i' < k` refl `C_normal\<^bsub>ML\<^esub> u'` `pure t'` this] show ?thesis .
+        from less(1)[OF `i' < k` refl `C_normal\<^sub>M\<^sub>L u'` `pure t'` this] show ?thesis .
       qed
     qed
   qed
@@ -2336,7 +2336,7 @@ proof -
 qed
 
 lemma C_normal_ML_compile:
-  "pure t \<Longrightarrow> \<forall>i. C_normal\<^bsub>ML\<^esub>(\<sigma> i) \<Longrightarrow> C_normal\<^bsub>ML\<^esub> (compile t \<sigma>)"
+  "pure t \<Longrightarrow> \<forall>i. C_normal\<^sub>M\<^sub>L(\<sigma> i) \<Longrightarrow> C_normal\<^sub>M\<^sub>L (compile t \<sigma>)"
 by(induct t arbitrary: \<sigma>) (simp_all add: C_normal_ML_lift_ML)
 
 corollary nbe_normal:
@@ -2418,7 +2418,7 @@ proof(induct ts rule:linpats.induct)
 qed
 
 lemma no_match_ML_swap_rev:
-  "length ps = length vs \<Longrightarrow> no_match\<^bsub>ML\<^esub> ps (rev vs) \<Longrightarrow> no_match\<^bsub>ML\<^esub> (rev ps) vs"
+  "length ps = length vs \<Longrightarrow> no_match\<^sub>M\<^sub>L ps (rev vs) \<Longrightarrow> no_match\<^sub>M\<^sub>L (rev ps) vs"
 apply(clarsimp simp: no_match_ML.simps[of ps] no_match_ML.simps[of _ vs])
 apply(rule_tac x="size ps - i - 1" in exI)
 apply (fastforce simp:rev_nth)
@@ -2426,13 +2426,13 @@ done
 
 lemma no_match_ML_aux:
   "ALL v : set cvs. C\<^sub>Us v \<Longrightarrow> linpats ps \<Longrightarrow> size ps = size cvs \<Longrightarrow>
-  \<forall>\<sigma>. map (subst\<^bsub>ML\<^esub> \<sigma>) (map comp_pat ps) \<noteq> cvs \<Longrightarrow>
-  no_match\<^bsub>ML\<^esub> (map comp_pat ps) cvs"
+  \<forall>\<sigma>. map (subst\<^sub>M\<^sub>L \<sigma>) (map comp_pat ps) \<noteq> cvs \<Longrightarrow>
+  no_match\<^sub>M\<^sub>L (map comp_pat ps) cvs"
 apply(induct ps arbitrary: cvs rule:linpats.induct)
 apply(frule linpats_pattern)
 apply(subst (asm) linpats.simps) back
 apply auto
-apply(case_tac "ALL i<size ts. EX \<sigma>. subst\<^bsub>ML\<^esub> \<sigma> (comp_pat (ts!i)) = cvs!i")
+apply(case_tac "ALL i<size ts. EX \<sigma>. subst\<^sub>M\<^sub>L \<sigma> (comp_pat (ts!i)) = cvs!i")
  apply(clarsimp simp:Skolem_list_nth)
  apply(rename_tac "\<sigma>s")
  apply(erule_tac x="%x. (\<sigma>s!(THE i. i<size ts & x : fv(ts!i)))x" in allE)
@@ -2477,7 +2477,7 @@ apply(erule_tac x=nm' in meta_allE)
 apply(erule_tac x="ts'" in meta_allE)
 apply(erule_tac x="rev vs'" in meta_allE)
 apply simp
-apply(subgoal_tac "no_match\<^bsub>ML\<^esub> (map comp_pat ts') (rev vs')")
+apply(subgoal_tac "no_match\<^sub>M\<^sub>L (map comp_pat ts') (rev vs')")
  apply(rule no_match_ML_swap_rev)
   apply simp
  apply assumption
